cogent/examples/repeat/WordArrayScorres.thy
@@ -45,36 +45,122 @@ definition swa_put :: "('a WordArray, 32 word, 'a) WordArrayGetP \<Rightarrow> '
    in list_to_swa (arr[i:= v]))"
 end (* of overloading *)
 
-class cogent_S_val = 
-  fixes valrel :: "(funtyp, vabstyp) vabsfuns \<Rightarrow> 'a \<Rightarrow> (funtyp, vabstyp) vval \<Rightarrow> bool"
-
-instantiation bool :: cogent_S_val
-begin
-definition valrel_bool_def:
-"valrel \<xi> x x' \<equiv> (x' = VPrim (LBool x))"
-instance ..
-end
-
-instantiation prod :: (cogent_S_val, cogent_S_val) cogent_S_val
-begin
-definition valrel_prod_def:
-"valrel \<xi> x x' \<equiv> (\<exists>a b. x' = VProduct a b \<and> valrel \<xi> (prod.fst x) a \<and> valrel \<xi> (prod.snd x) b)"
-instance ..
-end
-
-instantiation WordArray :: (cogent_S_val) cogent_S_val
-begin
-definition valrel_WordArray_def:
-"valrel \<xi> x x' \<equiv> (\<exists>t xs xs'. x' = VAbstract (VWA t xs) \<and> xs' = swa_to_list x \<and> length xs = length xs' \<and> (\<forall>i < length xs. valrel \<xi> (xs' ! i) (xs ! i)))"
-instance ..
-end
-(*
 overloading
-  valRel_WordArrayUX \<equiv> valRel
+  valRel_WordArrayWord \<equiv> valRel
 begin
-definition valRel_WordArrayUX:
-"\<And>\<xi>' x v. valRel_WordArrayUX (\<xi>' :: (funtyp, vabstyp) vabsfuns) (x :: (('a::len8) word) WordArray) (v :: (funtyp, vabstyp) vval) \<equiv> 
-  (\<exists>t xs. v = VAbstract(VWA t xs) \<and> length xs = length x \<and> (\<forall>i < length xs. valRel \<xi>' (x ! i) (xs ! i)))"
+definition valRel_WordArrayWord:
+"\<And>\<xi>' x v. 
+  valRel_WordArrayWord (\<xi>' :: (funtyp, vabstyp) vabsfuns) (x :: (('a::len8) word) WordArray) (v :: (funtyp, vabstyp) vval) \<equiv> 
+    (if len_of TYPE('a) = 8 then 
+        \<exists>xs xs'. v = VAbstract (VWA (TPrim (Num U8)) xs) \<and> xs' = swa_to_list x \<and> length xs' = length xs \<and> (\<forall>i < length xs. (xs ! i) = VPrim (LU8 (ucast (xs' ! i))))
+      else if len_of TYPE('a) = 16 then 
+        \<exists>xs xs'. v = VAbstract (VWA (TPrim (Num U16)) xs) \<and> xs' = swa_to_list x \<and> length xs' = length xs \<and> (\<forall>i < length xs. (xs ! i) = VPrim (LU16 (ucast (xs' ! i))))
+      else if len_of TYPE('a) = 32 then 
+        \<exists>xs xs'. v = VAbstract (VWA (TPrim (Num U32)) xs) \<and> xs' = swa_to_list x \<and> length xs' = length xs \<and> (\<forall>i < length xs. (xs ! i) = VPrim (LU32 (ucast (xs' ! i))))
+      else if len_of TYPE('a) = 64 then 
+        \<exists>xs xs'. v = VAbstract (VWA (TPrim (Num U64)) xs) \<and> xs' = swa_to_list x \<and> length xs' = length xs \<and> (\<forall>i < length xs. (xs ! i) = VPrim (LU64 (ucast (xs' ! i))))
+      else False)"
 end
-*)
+
+sublocale level0_value \<subseteq> shallow l0v_typing
+  by (unfold_locales)
+
+sublocale WordArrayValue \<subseteq> shallow wa_abs_typing_v
+  by (unfold_locales)
+
+context WordArrayValue begin
+
+lemma wordarray_length_scorres:
+  "\<xi> ''wordarray_length'' =  vwa_length 
+    \<Longrightarrow> scorres (wordarray_length :: ('a :: len8) word WordArray \<Rightarrow> 32 word) (AFun ''wordarray_length'' ts) \<gamma> \<xi>"
+  apply (clarsimp simp: scorres_def)
+  apply (erule v_sem_afunE; clarsimp)
+  apply (erule notE)
+  unfolding vwa_length_def swa_length_def valRel_WordArrayWord
+  apply (clarsimp split: if_splits)
+  done
+
+lemma wordarray_get_u8_scorres:
+  "\<xi> ''wordarray_get'' =  vwa_get 
+    \<Longrightarrow> scorres (wordarray_get :: (8 word WordArray, 32 word, 8 word) WordArrayGetP \<Rightarrow> 8 word) (AFun ''wordarray_get'' ts) \<gamma> \<xi>"
+  apply (clarsimp simp: scorres_def)
+  apply (erule v_sem_afunE; clarsimp)
+  apply (erule notE)
+  unfolding vwa_get_def swa_get_def valRel_WordArrayWord valRel_records
+  apply (clarsimp split: if_splits simp: Let_def ucast_id valRel_records)
+  done
+
+lemma wordarray_get_u16_scorres:
+  "\<xi> ''wordarray_get'' =  vwa_get 
+    \<Longrightarrow> scorres (wordarray_get :: (16 word WordArray, 32 word, 16 word) WordArrayGetP \<Rightarrow> 16 word) (AFun ''wordarray_get'' ts) \<gamma> \<xi>"
+  apply (clarsimp simp: scorres_def)
+  apply (erule v_sem_afunE; clarsimp)
+  apply (erule notE)
+  unfolding vwa_get_def swa_get_def valRel_WordArrayWord valRel_records
+  apply (clarsimp split: if_splits simp: Let_def ucast_id valRel_records)
+  done
+
+lemma wordarray_get_u32_scorres:
+  "\<xi> ''wordarray_get'' =  vwa_get 
+    \<Longrightarrow> scorres (wordarray_get :: (32 word WordArray, 32 word, 32 word) WordArrayGetP \<Rightarrow> 32 word) (AFun ''wordarray_get'' ts) \<gamma> \<xi>"
+  apply (clarsimp simp: scorres_def)
+  apply (erule v_sem_afunE; clarsimp)
+  apply (erule notE)
+  unfolding vwa_get_def swa_get_def valRel_WordArrayWord valRel_records
+  apply (clarsimp split: if_splits simp: Let_def ucast_id valRel_records)
+  done
+
+lemma wordarray_get_u64_scorres:
+  "\<xi> ''wordarray_get'' =  vwa_get 
+    \<Longrightarrow> scorres (wordarray_get :: (64 word WordArray, 32 word, 64 word) WordArrayGetP \<Rightarrow> 64 word) (AFun ''wordarray_get'' ts) \<gamma> \<xi>"
+  apply (clarsimp simp: scorres_def)
+  apply (erule v_sem_afunE; clarsimp)
+  apply (erule notE)
+  unfolding vwa_get_def swa_get_def valRel_WordArrayWord valRel_records
+  apply (clarsimp split: if_splits simp: Let_def ucast_id valRel_records)
+  done
+
+lemma wordarray_put_u8_scorres:
+  "\<xi> ''wordarray_put'' =  vwa_put 
+    \<Longrightarrow> scorres (wordarray_put :: (8 word WordArray, 32 word, 8 word) WordArrayGetP \<Rightarrow> 8 word WordArray) (AFun ''wordarray_put'' ts) \<gamma> \<xi>"
+  apply (clarsimp simp: scorres_def)
+  apply (erule v_sem_afunE; clarsimp)
+  apply (erule notE)
+  unfolding vwa_put_def swa_put_def valRel_WordArrayWord valRel_records
+  apply (clarsimp split: if_splits simp: Let_def ucast_id valRel_records)
+  by (metis (no_types, hide_lams) nth_list_update_eq nth_list_update_neq)
+
+lemma wordarray_put_u16_scorres:
+  "\<xi> ''wordarray_put'' =  vwa_put 
+    \<Longrightarrow> scorres (wordarray_put :: (16 word WordArray, 32 word, 16 word) WordArrayGetP \<Rightarrow> 16 word WordArray) (AFun ''wordarray_put'' ts) \<gamma> \<xi>"
+  apply (clarsimp simp: scorres_def)
+  apply (erule v_sem_afunE; clarsimp)
+  apply (erule notE)
+  unfolding vwa_put_def swa_put_def valRel_WordArrayWord valRel_records
+  apply (clarsimp split: if_splits simp: Let_def ucast_id valRel_records)
+  by (metis (no_types, hide_lams) nth_list_update_eq nth_list_update_neq)
+
+lemma wordarray_put_u32_scorres:
+  "\<xi> ''wordarray_put'' =  vwa_put 
+    \<Longrightarrow> scorres (wordarray_put :: (32 word WordArray, 32 word, 32 word) WordArrayGetP \<Rightarrow> 32 word WordArray) (AFun ''wordarray_put'' ts) \<gamma> \<xi>"
+  apply (clarsimp simp: scorres_def)
+  apply (erule v_sem_afunE; clarsimp)
+  apply (erule notE)
+  unfolding vwa_put_def swa_put_def valRel_WordArrayWord valRel_records
+  apply (clarsimp split: if_splits simp: Let_def ucast_id valRel_records)
+  by (metis (no_types, hide_lams) nth_list_update_eq nth_list_update_neq)
+
+lemma wordarray_put_u64_scorres:
+  "\<xi> ''wordarray_put'' =  vwa_put 
+    \<Longrightarrow> scorres (wordarray_put :: (64 word WordArray, 32 word, 64 word) WordArrayGetP \<Rightarrow> 64 word WordArray) (AFun ''wordarray_put'' ts) \<gamma> \<xi>"
+  apply (clarsimp simp: scorres_def)
+  apply (erule v_sem_afunE; clarsimp)
+  apply (erule notE)
+  unfolding vwa_put_def swa_put_def valRel_WordArrayWord valRel_records
+  apply (clarsimp split: if_splits simp: Let_def ucast_id valRel_records)
+  by (metis (no_types, hide_lams) nth_list_update_eq nth_list_update_neq)
+
+end
+
+
 end
