cogent/examples/repeat/BinarySearchAsm.thy
@@ -1,14 +1,15 @@
-theory RepeatAssm
+theory BinarySearchAsm
   imports
-    RepeatUpdate
-    RepeatValue
-    RepeatMono
     RepeatCorres
     RepeatCorrespondence
+    RepeatMono
     RepeatScorres
-    "build/Generated_AllRefine"
+    WordArrayCorres
+    WordArrayCorrespondence
+    WordArrayMono
+    WordArrayScorres
+   "build/Generated_AllRefine"
 begin
-
 section "Function types wellformed"
 
 lemma proc_ctx_wellformed_\<Xi>:
@@ -27,6 +28,8 @@ lemma \<Xi>_simps:
   "\<Xi> ''repeat_0'' = repeat_0_type"
   "\<Xi> ''repeat_1'' = repeat_1_type"
   "\<Xi> ''repeat_2'' = repeat_2_type"
+  "\<Xi> ''wordarray_length_0'' = wordarray_length_0_type"
+  "\<Xi> ''wordarray_get_0'' = wordarray_get_0_type"
   apply (clarsimp simp: \<Xi>_def)+
   done
 
@@ -50,7 +53,10 @@ overloading \<xi>0 \<equiv> \<xi>_0
 begin
 definition \<xi>0 :: "(funtyp, abstyp, ptrtyp) uabsfuns"
   where
-"\<xi>0 f x y = False"
+"\<xi>0 f x y = 
+  (if f = ''wordarray_length_0'' then uwa_length x y
+   else if f = ''wordarray_get_0'' then uwa_get x y
+   else False)"
 end
 
 overloading \<xi>1 \<equiv> \<xi>_1
@@ -73,27 +79,39 @@ lemma \<xi>_1_simps:
 
 subsection "Preservation for abstract functions"
 
-context update_sem_init begin
+
+sublocale WordArrayUpdate \<subseteq> update_sem_init wa_abs_typing_u wa_abs_repr 
+  by (unfold_locales)
+
+context WordArrayUpdate begin
 
 text "If user proves for \<xi>n, we can derive \<xi>i for i < n" 
 
 lemma \<xi>_0_matchesu_\<Xi>:
-  "\<xi>_0 matches-u \<Xi>'"
+  "proc_env_matches_ptrs \<xi>_0  \<Xi>"
   unfolding proc_env_matches_ptrs_def \<xi>0_def
-  by clarsimp
+  apply clarsimp
+  apply (intro conjI impI;
+         simp add: \<Xi>_simps Generated_TypeProof.wordarray_get_0_type_def
+                   Generated_TypeProof.wordarray_length_0_type_def;
+         clarsimp)
+   apply (rule uwa_get_preservation; simp?)
+   apply (rule uwa_length_preservation; simp?)
+  done
  
 lemma \<xi>_1_matchesu_\<Xi>:
-  "\<xi>_1 matches-u \<Xi>"
+  "proc_env_matches_ptrs \<xi>_1 \<Xi>"
   unfolding proc_env_matches_ptrs_def \<xi>1_def
   apply clarsimp
   apply (intro conjI impI; clarsimp simp: \<Xi>_simps)
     apply (clarsimp simp: repeat_1_type_def repeat_0_type_def repeat_2_type_def;
            rule_tac urepeat_preservation[OF proc_ctx_wellformed_\<Xi> \<xi>_0_matchesu_\<Xi>];
            (simp add: Generated_TypeProof.abbreviated_type_defs))+
-  apply (cut_tac \<Xi>' = \<Xi> in  \<xi>_0_matchesu_\<Xi>[unfolded proc_env_matches_ptrs_def]; clarsimp split: prod.splits)
+  apply (cut_tac \<xi>_0_matchesu_\<Xi>[unfolded proc_env_matches_ptrs_def]; clarsimp split: prod.splits)
   apply (elim allE impE conjE; assumption?)
   apply blast
   done
+
 end (* of context *)
 
 subsection "Partial ordering on abstract functions"
@@ -102,16 +120,14 @@ text "These should be automatable"
 
 lemma \<xi>_0_le_\<xi>_1:
   "rel_leq \<xi>_0 \<xi>_1"
-  unfolding \<xi>0_def rel_leq_def
-  by simp
-
-lemma \<xi>_0_le_\<xi>_1':
-  "rel_leq \<xi>_0 \<xi>_1"
   unfolding \<xi>1_def rel_leq_def
   apply clarsimp
+  apply (rename_tac n ac bb ad bc)
   apply (rule_tac x = n in exI; simp?)
   apply (intro exI conjI impI; simp?)
-  oops
+  apply (simp add: \<xi>0_def)+
+  done
+
 subsection "Abstract functions are deterministic"
 
 text "If user proves for \<xi>n, we can derive \<xi>i for i < n" 
@@ -119,7 +135,10 @@ text "If user proves for \<xi>n, we can derive \<xi>i for i < n"
 lemma \<xi>_0_determ:
   "determ \<xi>_0"
   unfolding determ_def \<xi>0_def
-  by simp
+  apply simp
+  apply clarsimp
+  apply (rule conjI; clarsimp simp: uwa_get_determ uwa_length_determ)
+  done
 
 lemma \<xi>_1_determ:
   "determ \<xi>_1"
@@ -133,15 +152,21 @@ lemma \<xi>_1_determ:
 
 section "Abstract functions specifications for the monomorphic value semantics"
 
-context monomorph_sem begin
+sublocale WordArrayValue \<subseteq> monomorph_sem wa_abs_typing_v
+  by (unfold_locales)
+
+context WordArrayValue begin
 
 text "If user defines for \<xi>n, we can derive \<xi>i for i < n" 
 
-definition \<xi>m0 :: "'b \<Rightarrow> ('b, 'a) vval \<Rightarrow> ('b, 'a) vval \<Rightarrow> bool "
+definition \<xi>m0 :: "funtyp \<Rightarrow> (funtyp, vabstyp) vval \<Rightarrow> (funtyp, vabstyp) vval \<Rightarrow> bool "
   where
-"\<xi>m0 f x y = False"
+"\<xi>m0 f x y =
+  (if f = ''wordarray_length_0'' then vwa_length x y
+   else if f = ''wordarray_get_0'' then vwa_get x y
+   else False)"
 
-definition \<xi>m1 :: "funtyp \<Rightarrow> (funtyp, 'a) vval \<Rightarrow> (funtyp, 'a) vval \<Rightarrow> bool "
+definition \<xi>m1 :: "funtyp \<Rightarrow> (funtyp, vabstyp) vval \<Rightarrow> (funtyp, vabstyp) vval \<Rightarrow> bool "
   where
 "\<xi>m1 f x y = 
   (if f = ''repeat_0'' then vrepeat \<Xi> \<xi>m0 (acctyp \<Xi> f) (obsvtyp \<Xi> f) x y 
@@ -154,19 +179,26 @@ subsection "Preservation for abstract functions"
 text "If user proves for \<xi>n, we can derive \<xi>i for i < n" 
 
 lemma \<xi>m0_matches_\<Xi>:
-  "\<xi>m0 matches \<Xi>'"
+  "proc_env_matches \<xi>m0  \<Xi>"
   unfolding proc_env_matches_def \<xi>m0_def
-  by clarsimp
+  apply clarsimp
+  apply (intro conjI impI;
+         simp add: \<Xi>_simps Generated_TypeProof.wordarray_get_0_type_def
+                   Generated_TypeProof.wordarray_length_0_type_def;
+         clarsimp)
+   apply (rule vwa_get_preservation; simp?)
+  apply (rule vwa_length_preservation; simp?)
+  done
 
 lemma \<xi>m1_matches_\<Xi>:
-  "\<xi>m1 matches \<Xi>"
+  "proc_env_matches \<xi>m1 \<Xi>"
   unfolding proc_env_matches_def \<xi>m1_def
   apply clarsimp
   apply (intro conjI impI)
     apply (clarsimp simp: \<Xi>_simps repeat_1_type_def repeat_0_type_def repeat_2_type_def;
            rule vrepeat_preservation[OF proc_ctx_wellformed_\<Xi> \<xi>m0_matches_\<Xi>];
            (simp add: Generated_TypeProof.abbreviated_type_defs)?)+
-  apply (cut_tac \<Xi>' = \<Xi> in \<xi>m0_matches_\<Xi>[unfolded proc_env_matches_def]; clarsimp split: prod.splits)
+  apply (cut_tac \<xi>m0_matches_\<Xi>[unfolded proc_env_matches_def]; clarsimp split: prod.splits)
   done
 
 subsection "Partial ordering on abstract functions"
@@ -175,8 +207,13 @@ text "Should be automatable"
 
 lemma \<xi>m0_le_\<xi>m1:
   "rel_leq \<xi>m0 \<xi>m1"
-  unfolding \<xi>m0_def rel_leq_def
-  by simp
+  unfolding \<xi>m1_def rel_leq_def
+  apply clarsimp
+  apply (rename_tac n a b)
+  apply (rule_tac x = n in exI; simp?)
+  apply (intro exI conjI impI; simp?)
+  apply (simp add: \<xi>m0_def)+
+  done
 
 subsection "Abstract functions are deterministic"
 
@@ -185,7 +222,9 @@ text "If user proves for \<xi>n, we can derive \<xi>i for i < n"
 lemma \<xi>m0_determ:
   "determ \<xi>m0"
   unfolding determ_def \<xi>m0_def
-  by simp
+  apply clarsimp
+  apply (rule conjI; clarsimp simp: vwa_get_determ vwa_length_determ)
+  done
 
 lemma \<xi>m1_determ:
   "determ \<xi>m1"
@@ -202,11 +241,14 @@ section "Abstract functions specifications for the polymorphic value semantics"
 
 text "If user defines \<xi>n, we can derive \<xi>i for i < n" 
 
-definition \<xi>p0 :: "'b \<Rightarrow> ('b, 'c) vval \<Rightarrow> ('b, 'c) vval \<Rightarrow> bool"
+definition \<xi>p0 :: "funtyp \<Rightarrow> (funtyp, vabstyp) vval \<Rightarrow> (funtyp, vabstyp) vval \<Rightarrow> bool"
   where
-"\<xi>p0 f x y = False"
+"\<xi>p0 f x y =
+  (if f = ''wordarray_length'' then vwa_length x y
+   else if f = ''wordarray_get'' then vwa_get x y
+   else False)"
 
-definition \<xi>p1 :: "funtyp \<Rightarrow> (funtyp, 'c) vval \<Rightarrow> (funtyp, 'c) vval \<Rightarrow> bool"
+definition \<xi>p1 :: "funtyp \<Rightarrow> (funtyp, vabstyp) vval \<Rightarrow> (funtyp, vabstyp) vval \<Rightarrow> bool"
   where
 "\<xi>p1 f x y = (if f = ''repeat'' then prepeat \<xi>p0 x y else \<xi>p0 f x y)"
 
@@ -216,8 +258,13 @@ text "Should be automatable"
 
 lemma \<xi>p0_le_\<xi>p1:
   "rel_leq \<xi>p0 \<xi>p1"
-  unfolding \<xi>p0_def rel_leq_def
-  by simp
+  unfolding \<xi>p1_def rel_leq_def
+  apply clarsimp
+  apply (rename_tac n a b)
+  apply (rule_tac x = n in exI; simp?)
+  apply (intro exI conjI impI; simp?)
+  apply (simp add: \<xi>p0_def)+
+  done
 
 subsection "Abstract functions are deterministic"
 
@@ -226,7 +273,9 @@ text "If user proves for \<xi>n, we can derive \<xi>i for i < n"
 lemma \<xi>p0_determ:
   "determ \<xi>p0"
   unfolding determ_def \<xi>p0_def
-  by simp
+  apply clarsimp
+  apply (rule conjI; clarsimp simp: vwa_get_determ vwa_length_determ)
+  done
 
 lemma \<xi>p1_determ:
   "determ \<xi>p1"
@@ -321,25 +370,122 @@ lemma myexp_repeat_corres:
 
 end (* of context *)
 
-section "Correspondence between abstract functions in the update and value semantics"
+sublocale WordArrayUpdate \<subseteq> Generated _ wa_abs_typing_u wa_abs_repr
+  by (unfold_locales)
 
-context correspondence_init begin
+sublocale WordArrayUpdate \<subseteq> update_sem_init wa_abs_typing_u wa_abs_repr
+  by (unfold_locales)
+
+context WordArrayUpdate begin
+
+lemma wordarray_length_0_corres:
+  "\<And>i \<gamma> v' \<Gamma>' \<sigma> st.
+    \<lbrakk>i < length \<gamma>; val_rel (\<gamma> ! i) v';
+     \<Gamma>' ! i = Some (fst (snd (\<Xi> ''wordarray_length_0'')))\<rbrakk>
+    \<Longrightarrow> corres state_rel (App (AFun ''wordarray_length_0'' []) (Var i)) (do x <- wordarray_length_0' v';
+        gets (\<lambda>s. x)
+     od)
+         \<xi>_0 \<gamma> \<Xi> \<Gamma>' \<sigma> st"
+  apply (rule_tac is_v = is_valid and h = heap and
+      l_c = WordArray_u32_C.len_C and v_c = WordArray_u32_C.values_C 
+      in cwa_length_corres_base; simp add: \<Xi>_simps wordarray_length_0_type_def fun_eq_iff;
+      clarsimp simp: state_rel_def heap_rel_def heap_rel_ptr_meta type_rel_simp \<xi>1_def \<xi>0_def val_rel_simp
+      wordarray_length_0'_def cwa_length_def unknown_bind_ignore is_valid_simp heap_simp)
+  done
+
+thm  corres_rel_leqD[OF \<xi>_0_le_\<xi>_1 wordarray_length_0_corres]
+
+lemma wordarray_get_0'_simp:
+  "wordarray_get_0' = cwa_get is_valid_WordArray_u32_C heap_WordArray_u32_C is_valid_w32 heap_w32 t1_C.arr_C t1_C.idx_C t1_C.val_C WordArray_u32_C.len_C WordArray_u32_C.values_C"
+  unfolding wordarray_get_0'_def[polish] cwa_get_def
+  by (simp add: unknown_bind_ignore)
+
+lemma wordarray_get_0_corres:
+  "\<And>i \<gamma> v' \<Gamma>' \<sigma> st.
+    \<lbrakk>i < length \<gamma>; val_rel (\<gamma> ! i) v';
+     \<Gamma>' ! i = Some (fst (snd (\<Xi> ''wordarray_get_0'')))\<rbrakk>
+    \<Longrightarrow> corres state_rel (App (AFun ''wordarray_get_0'' []) (Var i)) (do x <- wordarray_get_0' v';
+        gets (\<lambda>s. x)
+     od)
+         \<xi>_0 \<gamma> \<Xi> \<Gamma>' \<sigma> st"
+  apply (rule_tac  cwa_get_corres_base[rotated -1, OF  wordarray_get_0'_simp]; 
+      simp add: \<Xi>_simps wordarray_get_0_type_def fun_eq_iff;
+      clarsimp simp: state_rel_def heap_rel_def heap_rel_ptr_meta type_rel_simp \<xi>1_def \<xi>0_def val_rel_simp
+      wordarray_length_0'_def cwa_length_def unknown_bind_ignore is_valid_simp heap_simp)
+  done
+
+lemma repeat_2'_simp:
+  "repeat_2' = crepeat t12_C.n_C t12_C.stop_C t12_C.step_C t12_C.acc_C t12_C.obsv_C t9_C.acc_C t9_C.acc_C_update t9_C.obsv_C_update dispatch_t10' dispatch_t11'"
+  unfolding crepeat_def[polish] repeat_2'_def[simplified L2polish, polish]
+  apply clarsimp
+  done
+
+
+
+lemma binarySearch_repeat_corres:
+  "\<And>v' i \<gamma> \<Gamma> \<sigma> s.
+    \<lbrakk>t12_C.stop_C v' = FUN_ENUM_searchStop; t12_C.step_C v' = FUN_ENUM_searchNext; i < length \<gamma>; val_rel (\<gamma> ! i) v';
+     \<Gamma> ! i = Some (fst (snd repeat_2_type))\<rbrakk>
+    \<Longrightarrow> corres state_rel (App (AFun ''repeat_2'' []) (Var i)) (do x <- repeat_2' v';
+ gets (\<lambda>s. x)
+                                                               od)
+         \<xi>_1 \<gamma> \<Xi> \<Gamma> \<sigma> s"
+  apply simp
+  apply (subst (asm) \<Xi>_simps[symmetric])
+  apply (cut_tac uv = "\<gamma>!i" and x = v' in val_rel_t12_C_def)
+  apply (rule crepeat_corres_bang_fun_fun[
+        where o1C = t9_C.obsv_C and \<xi>' = \<xi>_0,
+        OF _ _ _ _  _ _ _  _ _ \<xi>_0_le_\<xi>_1 \<xi>_1_determ _
+        searchStop_typecorrect'[simplified Generated_TypeProof.searchStop_type_def fst_conv snd_conv]
+        searchNext_typecorrect'[simplified Generated_TypeProof.searchNext_type_def fst_conv snd_conv]
+        _ _ _ _ _ _ _ _ repeat_2'_simp]; 
+        (simp add: \<Xi>_simps \<xi>_1_simps
+            Generated_TypeProof.repeat_2_type_def Generated_TypeProof.abbreviated_type_defs)?)
+        apply (clarsimp simp: cogent_function_val_rel untyped_func_enum_defs val_rel_simp)
+     apply (subst Generated_TypeProof.abbreviated_type_defs[symmetric])+
+     apply (rule corres_app_concrete[simplified]; simp?)
+     apply (simp add: dispatch_t10'_def unknown_bind_ignore)
+     apply (erule corres_searchStop[folded \<Xi>_def, simplified fst_conv snd_conv Generated_TypeProof.searchStop_type_def])
+    apply (subst Generated_TypeProof.abbreviated_type_defs[symmetric])+
+    apply (rule corres_app_concrete[simplified]; simp?)
+    apply (simp add: dispatch_t11'_def unknown_bind_ignore)
+    apply (rule corres_searchNext[folded \<Xi>_def, simplified fst_conv snd_conv Generated_TypeProof.searchNext_type_def])
+     apply (rule wordarray_get_0_corres; (simp add: \<Xi>_simps)?)
+    apply simp
+   apply (clarsimp simp: val_rel_simp)
+  apply (clarsimp simp: val_rel_simp)
+  done
+
+
+end (* of context *)
+
+
+section "Correspondence between abstract functions in the update and value semantics"
+sublocale WordArray \<subseteq> correspondence_init upd.wa_abs_repr val.wa_abs_typing_v upd.wa_abs_typing_u wa_abs_upd_val
+  by (unfold_locales)
+term \<xi>m0
+
+context WordArray begin
 
 lemma \<xi>_0_\<xi>m0_matchesuv_\<Xi>:
-  "\<xi>_0 \<sim> \<xi>m0 matches-u-v \<Xi>'"
-  unfolding proc_env_u_v_matches_def \<xi>0_def \<xi>m0_def
-  by clarsimp
+  "proc_env_u_v_matches \<xi>_0 val.\<xi>m0  \<Xi>"
+  unfolding proc_env_u_v_matches_def \<xi>0_def val.\<xi>m0_def
+  apply clarsimp
+  apply (rule conjI; clarsimp simp: \<Xi>_simps wordarray_get_0_type_def wordarray_length_0_type_def)
+   apply (rule uvwa_get_monocorrespond_upward_propagation; simp?)
+  apply (rule uvwa_length_monocorrespond_upward_propagation; simp?)
+  done
 
 lemma \<xi>_1_\<xi>m1_matchesuv_\<Xi>:
-  "\<xi>_1 \<sim> \<xi>m1 matches-u-v \<Xi>"
-  unfolding proc_env_u_v_matches_def \<xi>1_def \<xi>m1_def
+  "proc_env_u_v_matches \<xi>_1 val.\<xi>m1 \<Xi>"
+  unfolding proc_env_u_v_matches_def \<xi>1_def val.\<xi>m1_def
   apply clarsimp
   apply (intro conjI impI; clarsimp)
     apply (subst (asm) \<Xi>_def;
            clarsimp simp: Generated_TypeProof.repeat_1_type_def Generated_TypeProof.repeat_0_type_def Generated_TypeProof.repeat_2_type_def;
            rule uvrepeat_monocorrespond_upward_propagation[OF proc_ctx_wellformed_\<Xi> \<xi>_0_\<xi>m0_matchesuv_\<Xi>];
            (simp add: Generated_TypeProof.abbreviated_type_defs)?)+
-  apply (cut_tac  \<xi>_0_\<xi>m0_matchesuv_\<Xi>[where \<Xi>' = \<Xi>, unfolded proc_env_u_v_matches_def, simplified])
+  apply (cut_tac \<xi>_0_\<xi>m0_matchesuv_\<Xi>[unfolded proc_env_u_v_matches_def, simplified])
   apply (clarsimp split: prod.splits)
   apply (elim allE impE conjE; assumption?)
   apply blast
@@ -349,12 +495,17 @@ end (* of context *)
 
 section "Monomorphisation of abstract functions"
 
-context monomorph_sem begin
+context WordArrayValue begin
 
 lemma rename_mono_prog_\<xi>m0_\<xi>p0:
-  "rename_mono_prog rename' \<Xi>' \<xi>m0 \<xi>p0"
+  "rename_mono_prog rename \<Xi> \<xi>m0 \<xi>p0"
   unfolding rename_mono_prog_def \<xi>m0_def \<xi>p0_def
-  by clarsimp
+  apply clarsimp
+  apply (intro conjI impI; clarsimp?)
+    apply (subst (asm) rename_def,
+           clarsimp simp: assoc_lookup.simps vwa_get_monoexpr_correct vwa_length_monoexpr_correct
+                    split: if_splits)+
+  done
 
 lemma rename_mono_prog_\<Xi>_\<xi>m1_\<xi>p1:
   "rename_mono_prog rename \<Xi> \<xi>m1 \<xi>p1"
@@ -364,41 +515,61 @@ lemma rename_mono_prog_\<Xi>_\<xi>m1_\<xi>p1:
     apply (subst (asm) rename_def,
            clarsimp simp: assoc_lookup.simps split: if_splits;
            rule prepeat_monoexpr_correct[OF _ \<xi>m0_matches_\<Xi> rename_mono_prog_\<xi>m0_\<xi>p0]; simp?)+
-  apply (cut_tac rename' = rename and \<Xi>' = \<Xi> in rename_mono_prog_\<xi>m0_\<xi>p0[unfolded rename_mono_prog_def];
+  apply (cut_tac rename_mono_prog_\<xi>m0_\<xi>p0[unfolded rename_mono_prog_def];
       clarsimp simp: \<xi>m0_matches_\<Xi>)
   apply (elim allE impE, assumption, clarsimp)
   apply (intro exI conjI impI; simp?)
-  apply (clarsimp simp: \<xi>m0_def)
+  apply (clarsimp simp: \<xi>m0_def rename_def assoc_lookup.simps split: if_splits)
   done
 
 end (* of context *)
 
 section "Correspondence between shallow and polymorphic value semantics"
 
-lemma (in shallow) scorres_repeat:
+sublocale WordArrayValue \<subseteq> shallow wa_abs_typing_v
+  by (unfold_locales)
+
+lemma (in WordArrayValue) scorres_repeat:
   "scorres repeat (AFun ''repeat'' ts) \<gamma> \<xi>p1"
   by (rule repeat_scorres[OF \<xi>p0_le_\<xi>p1]; simp add: \<xi>p1_def fun_eq_iff)
 
 section "All refine"
 
-lemmas (in Generated_cogent_shallow) corres_shallow_C_log2step_concrete = corres_shallow_C_log2step
-  [OF _ rename_mono_prog_\<xi>m0_\<xi>p0 _ _ proc_ctx_wellformed_\<Xi> \<xi>m0_matches_\<Xi>]
+sublocale WordArray \<subseteq> Generated_cogent_shallow _ upd.wa_abs_repr val.wa_abs_typing_v upd.wa_abs_typing_u wa_abs_upd_val
+  by (unfold_locales)
 
-lemmas (in Generated_cogent_shallow) corres_shallow_C_log2stop_concrete = corres_shallow_C_log2stop
-  [OF _ rename_mono_prog_\<xi>m0_\<xi>p0 _ _ proc_ctx_wellformed_\<Xi> \<xi>m0_matches_\<Xi>]
+lemmas (in WordArray) corres_shallow_C_log2step_concrete = corres_shallow_C_log2step
+  [OF _ val.rename_mono_prog_\<xi>m0_\<xi>p0 _ _ proc_ctx_wellformed_\<Xi> val.\<xi>m0_matches_\<Xi>]
 
-lemmas (in Generated_cogent_shallow) corres_shallow_C_mylog2_concrete = corres_shallow_C_mylog2
-  [folded \<Xi>_def, OF _ _ rename_mono_prog_\<Xi>_\<xi>m1_\<xi>p1 _ _ proc_ctx_wellformed_\<Xi> \<xi>m1_matches_\<Xi>,
-   simplified, OF mylog2_repeat_corres[simplified]]
+lemmas (in WordArray) corres_shallow_C_log2stop_concrete = corres_shallow_C_log2stop
+  [OF _ val.rename_mono_prog_\<xi>m0_\<xi>p0 _ _ proc_ctx_wellformed_\<Xi> val.\<xi>m0_matches_\<Xi>]
 
-lemmas (in Generated_cogent_shallow) corres_shallow_C_expstep_concrete = corres_shallow_C_expstep
-  [OF _ rename_mono_prog_\<xi>m0_\<xi>p0 _ _ proc_ctx_wellformed_\<Xi> \<xi>m0_matches_\<Xi>]
+lemmas (in WordArray) corres_shallow_C_mylog2_concrete = corres_shallow_C_mylog2
+  [folded \<Xi>_def, OF _ _ val.rename_mono_prog_\<Xi>_\<xi>m1_\<xi>p1 _ _ proc_ctx_wellformed_\<Xi> val.\<xi>m1_matches_\<Xi>,
+   simplified, OF upd.mylog2_repeat_corres[simplified], simplified, simplified \<Xi>_simps, simplified]
 
-lemmas (in Generated_cogent_shallow) corres_shallow_C_expstop_concrete = corres_shallow_C_expstop
-  [OF _ rename_mono_prog_\<xi>m0_\<xi>p0 _ _ proc_ctx_wellformed_\<Xi> \<xi>m0_matches_\<Xi>]
+lemmas (in WordArray) corres_shallow_C_expstep_concrete = corres_shallow_C_expstep
+  [OF _ val.rename_mono_prog_\<xi>m0_\<xi>p0 _ _ proc_ctx_wellformed_\<Xi> val.\<xi>m0_matches_\<Xi>]
 
-lemmas (in Generated_cogent_shallow) corres_shallow_C_myexp_concrete = corres_shallow_C_myexp
-  [folded \<Xi>_def, OF _ _ rename_mono_prog_\<Xi>_\<xi>m1_\<xi>p1 _ _ proc_ctx_wellformed_\<Xi> \<xi>m1_matches_\<Xi>,
-   simplified, OF myexp_repeat_corres[simplified]]
+lemmas (in WordArray) corres_shallow_C_expstop_concrete = corres_shallow_C_expstop
+  [OF _ val.rename_mono_prog_\<xi>m0_\<xi>p0 _ _ proc_ctx_wellformed_\<Xi> val.\<xi>m0_matches_\<Xi>]
+
+lemmas (in WordArray) corres_shallow_C_myexp_concrete = corres_shallow_C_myexp
+  [folded \<Xi>_def, OF _ _ val.rename_mono_prog_\<Xi>_\<xi>m1_\<xi>p1 _ _ proc_ctx_wellformed_\<Xi> val.\<xi>m1_matches_\<Xi>,
+   simplified, OF upd.myexp_repeat_corres[simplified], simplified, simplified \<Xi>_simps, simplified]
+
+lemmas (in WordArray) corres_shallow_C_searchStop_concrete = corres_shallow_C_searchStop
+  [OF _ val.rename_mono_prog_\<xi>m0_\<xi>p0 _ _ proc_ctx_wellformed_\<Xi> val.\<xi>m0_matches_\<Xi>]
+
+lemmas (in WordArray) corres_shallow_C_searchNext_concrete = corres_shallow_C_searchNext
+  [folded \<Xi>_def, OF _ _ val.rename_mono_prog_\<xi>m0_\<xi>p0 _ _ proc_ctx_wellformed_\<Xi> val.\<xi>m0_matches_\<Xi>,
+   simplified, OF upd.wordarray_get_0_corres[simplified], simplified, simplified \<Xi>_simps, simplified]
+
+lemmas (in WordArray) corres_shallow_C_binarySearch_concrete = corres_shallow_C_binarySearch
+  [folded \<Xi>_def, OF _ _ _ val.rename_mono_prog_\<xi>m0_\<xi>p0 _ _ proc_ctx_wellformed_\<Xi> val.\<xi>m0_matches_\<Xi>,
+   simplified, 
+   OF _ upd.binarySearch_repeat_corres[simplified], simplified,
+   OF upd.corres_rel_leqD[OF \<xi>_0_le_\<xi>_1 upd.wordarray_length_0_corres[simplified]],
+   simplified, simplified \<Xi>_simps, simplified]
 
 end
