cogent/examples/repeat/WordArrayCorres.thy
@@ -1,0 +1,174 @@
+theory WordArrayCorres
+  imports
+    WordArrayUpdate
+    CorresHelper
+    CogentTypingHelper
+    "build/Generated_CorresSetup"
+begin
+
+sublocale WordArrayUpdate \<subseteq> update_sem_init wa_abs_typing_u wa_abs_repr
+  by (unfold_locales)
+
+context WordArrayUpdate begin
+
+definition cwa_length
+  where
+"cwa_length is_v h l_c a \<equiv>
+    do _ <- guard (\<lambda>s. is_v s a);
+       _ <- guard (\<lambda>s. is_v s a);
+       gets (\<lambda>s. SCAST(32 signed \<rightarrow> 32) (l_c (h s a)))
+    od"
+
+lemma cwa_length_corres_base:
+  assumes \<gamma>len: "i < length \<gamma>"
+  and     valrel: "val_rel (\<gamma> ! i) (v' :: ('a :: cogent_C_val) ptr)"
+  and     \<Gamma>i: "\<Gamma> ! i = Some (fst (snd (\<Xi>' name)))"
+  and     \<Xi>name: "\<Xi>' name = ([], TCon ''WordArray'' [t] (Boxed ReadOnly ptrl), TPrim (Num U32))"
+  and     \<xi>name: "\<xi>' name = uwa_length"
+  and     srel: "\<And>x y. (x, y) \<in> state_rel \<Longrightarrow> (\<forall>(p :: ('a :: cogent_C_val) ptr) uv. heap_rel_meta is_v h x y p)"
+  and     trel: "type_rel (RCon ''WordArray'' [type_repr t]) TYPE('a)"
+  and     vrel: "\<And>uv (cv :: 'a). 
+                  val_rel uv cv = 
+                    (\<exists>len arr. uv = UAbstract (UWA t len arr) \<and>
+                      len = (SCAST(32 signed \<rightarrow> 32)(l_c cv)) \<and> arr = ptr_val (v_c cv))"
+  and     cfundef: "cfun = cwa_length is_v h l_c"
+shows
+  "corres state_rel (App (AFun name []) (Var i))
+    (do x <- cfun v'; gets (\<lambda>s. x) od)
+     \<xi>' \<gamma> \<Xi>' \<Gamma> \<sigma> s"
+proof (rule absfun_corres[OF _ \<gamma>len valrel])
+  show "abs_fun_rel \<Xi>' state_rel name \<xi>' cfun \<sigma> s (\<gamma> ! i) v'"
+    apply (subst abs_fun_rel_def)
+    apply (clarsimp simp: cfundef \<Xi>name \<xi>name uwa_length_def)
+    apply (erule u_t_tconE; clarsimp simp: val_rel_ptr_def)
+    apply (frule wa_abs_typing_u_elims(1); clarsimp)
+    apply (cut_tac srel; simp?)
+    apply (erule_tac x = v' in allE; clarsimp simp: heap_rel_meta_def wa_abs_repr_def trel)
+    apply (rule conjI; monad_eq simp: cwa_length_def)
+    apply (clarsimp simp: val_rel_word_def vrel is_signed_bit0_def word_bits_size word_bits_def)
+    done
+next
+  show "\<Gamma> ! i = Some (fst (snd (\<Xi>' name)))"
+    by (simp add: \<Gamma>i)
+qed
+
+definition cwa_get
+  where
+"cwa_get is_v h is_vw hw p_c i_c v_c l_c vs_c a \<equiv>
+    do _ <- guard (\<lambda>s. is_v s (p_c a));
+       _ <- guard (\<lambda>s. is_v s (p_c a));
+       condition (\<lambda>s. SCAST(32 signed \<rightarrow> 32) (l_c (h s (p_c a))) \<le> i_c a)
+         (return (v_c a))
+         (do _ <-
+             guard
+              (\<lambda>s. is_v s (p_c a) \<and>
+                   is_vw s (vs_c (h s (p_c a)) +\<^sub>p uint (i_c a)));
+             _ <- guard (\<lambda>s. is_v s (p_c a));
+             _ <-
+             guard
+              (\<lambda>s. is_v s (p_c a) \<and>
+                   is_vw s (vs_c (h s (p_c a)) +\<^sub>p uint (i_c a)));
+             gets (\<lambda>s. hw s (vs_c (h s (p_c a)) +\<^sub>p uint (i_c a)))
+          od)
+    od"
+
+lemma ptr_val_add: 
+  "ptr_val (p :: ('a :: c_type) ptr) + of_nat (size_of TYPE('a)) * x = ptr_val (p +\<^sub>p uint x)"
+  apply (simp add: ptr_add_def mult.commute)
+  done
+
+
+lemma cwa_get_corres_base:
+  assumes \<gamma>len: "i < length \<gamma>"
+  and     valrel: "val_rel (\<gamma> ! i) (v' :: ('b :: cogent_C_val))"
+  and     \<Gamma>i: "\<Gamma> ! i = Some (fst (snd (\<Xi>' name)))"
+  and     \<Xi>name: "\<Xi>' name = ([], TRecord [
+                    (''arr'', TCon ''WordArray'' [t] (Boxed ReadOnly ptrl), Present),
+                    (''idx'', TPrim (Num U32), Present),
+                    (''val'', t, Present)] Unboxed, t)"
+  and     \<xi>name: "\<xi>' name = uwa_get"
+  and     srel: "\<And>x y. (x, y) \<in> state_rel \<Longrightarrow> 
+                  (\<forall>(p :: ('a :: cogent_C_val) ptr) uv. heap_rel_meta is_v h x y p) \<and>
+                  (\<forall>(p :: ('c :: cogent_C_val) ptr) uv. heap_rel_meta is_vw hw x y p)"
+  and     trela: "type_rel (RCon ''WordArray'' [type_repr t]) TYPE('a)"
+  and     trelc: "type_rel (type_repr t) TYPE('c)"
+  and     vrela: "\<And>uv (cv :: 'a). 
+                  val_rel uv cv = 
+                    (\<exists>len arr. uv = UAbstract (UWA t len arr) \<and>
+                      len = (SCAST(32 signed \<rightarrow> 32)(l_c cv)) \<and> arr = ptr_val (vs_c cv))"
+  and     vrelb: "\<And>uv (cv :: 'b). 
+                  val_rel uv cv = 
+                    (\<exists>p i v. uv = URecord [p, i, v] \<and> val_rel (prod.fst p) (p_c cv) \<and>
+                      val_rel (prod.fst i) (i_c cv) \<and> val_rel (prod.fst v) (v_c cv))"
+  and     sizet: "size_of_type t = of_nat (size_of TYPE('c))"
+  and     cfundef: "cfun = cwa_get is_v h is_vw hw p_c i_c v_c l_c vs_c"
+shows
+  "corres state_rel (App (AFun name []) (Var i))
+    (do x <- cfun v'; gets (\<lambda>s. x) od)
+     \<xi>' \<gamma> \<Xi>' \<Gamma> \<sigma> s"
+proof (rule absfun_corres[OF _ \<gamma>len valrel])
+  show "abs_fun_rel \<Xi>' state_rel name \<xi>' cfun \<sigma> s (\<gamma> ! i) v'"
+    apply (subst abs_fun_rel_def)
+    apply (clarsimp simp: cfundef \<Xi>name \<xi>name vrelb val_rel_ptr_def val_rel_word_def 
+                          is_signed_bit0_def word_bits_size word_bits_def ucast_id)
+    apply (erule u_t_recE; clarsimp)
+    apply (erule u_t_r_consE; clarsimp)+
+    apply (erule u_t_r_emptyE; clarsimp)
+    apply (erule u_t_tconE; clarsimp)
+    apply (erule u_t_primE)
+    apply (drule_tac t = "lit_type _" in sym; clarsimp)
+    apply (cut_tac srel; simp?)
+    apply clarsimp
+    apply (frule wa_abs_typing_u_elims(1); clarsimp)
+    apply (drule (1) all_heap_rel_ptrD; clarsimp simp: trela wa_abs_repr_def vrela split: atyp.splits)
+    apply (rule conjI)
+     apply (monad_eq simp: cwa_get_def)
+     apply (frule wa_abs_typing_u_elims(5))
+     apply (erule_tac x = "i_c v'" in allE; clarsimp simp: not_le sizet)
+     apply (simp add: ptr_val_add)
+     apply (drule (1) all_heap_rel_ptrD)
+      apply (drule l0.type_repr_uval_repr; simp add: l0_eq_uval_repr trelc)
+     apply clarsimp
+    apply clarsimp
+    apply (monad_eq simp: cwa_get_def)
+    apply (rule_tac x = \<sigma> in exI)
+    apply (case_tac "SCAST(32 signed \<rightarrow> 32) (l_c (h s (p_c v'))) \<le> i_c v'"; clarsimp)
+     apply (rename_tac x rb wb rc)
+     apply (rule_tac x = x in exI)
+     apply clarsimp
+     apply (fastforce simp: uwa_get_def)
+    apply (frule wa_abs_typing_u_elims(5))
+    apply (erule_tac x = "i_c v'" in allE; clarsimp simp: not_le sizet)
+    apply (simp add: ptr_val_add)
+    apply (drule (1) all_heap_rel_ptrD)
+     apply (drule l0.type_repr_uval_repr; simp add: l0_eq_uval_repr trelc)
+    apply clarsimp
+    apply (rename_tac xa)
+    apply (rule_tac x = xa in exI)
+    apply (clarsimp simp: uwa_get_def sizet ptr_val_add)
+    done
+next
+  show "\<Gamma> ! i = Some (fst (snd (\<Xi>' name)))"
+    by (simp add: \<Gamma>i)
+qed
+
+end (* of context *)
+
+sublocale WordArrayUpdate \<subseteq> Generated _ wa_abs_typing_u wa_abs_repr
+  by (unfold_locales)
+
+context WordArrayUpdate begin
+
+lemma
+  "wordarray_length_0' = cwa_length is_valid heap len_C"
+  unfolding wordarray_length_0'_def cwa_length_def
+  by (clarsimp simp: is_valid_simp heap_simp unknown_bind_ignore) 
+
+
+lemma
+  "wordarray_get_0' = cwa_get is_valid heap is_valid_w32 heap_w32 arr_C idx_C val_C len_C values_C"
+  unfolding wordarray_get_0'_def cwa_get_def
+  by (clarsimp simp: is_valid_simp heap_simp unknown_bind_ignore) 
+
+end
+end
