cogent/examples/repeat/build/Generated_TypeProof.thy
@@ -21,29 +21,35 @@ where
 definition
   abbreviatedType3 :: " Cogent.type"
 where
-  "abbreviatedType3 \<equiv> TRecord [(''acc'', (abbreviatedType1, Present)), (''obsv'', (abbreviatedType2, Present))] Unboxed"
+  "abbreviatedType3 \<equiv> TRecord [(''p1'', (TPrim (Num U32), Present)), (''p2'', (TPrim (Num U32), Present)), (''p3'', (TPrim Bool, Present))] Unboxed"
 
 definition
   abbreviatedType4 :: " Cogent.type"
 where
-  "abbreviatedType4 \<equiv> TRecord [(''p1'', (TPrim (Num U64), Present)), (''p2'', (TPrim (Num U64), Present))] Unboxed"
+  "abbreviatedType4 \<equiv> TRecord [(''acc'', (abbreviatedType3, Present)), (''obsv'', (abbreviatedType2, Present))] Unboxed"
 
 definition
   abbreviatedType5 :: " Cogent.type"
 where
-  "abbreviatedType5 \<equiv> TRecord [(''acc'', (abbreviatedType4, Present)), (''obsv'', (TPrim (Num U64), Present))] Unboxed"
+  "abbreviatedType5 \<equiv> TRecord [(''p1'', (TPrim (Num U64), Present)), (''p2'', (TPrim (Num U64), Present))] Unboxed"
 
 definition
   abbreviatedType6 :: " Cogent.type"
 where
-  "abbreviatedType6 \<equiv> TRecord [(''acc'', (TPrim (Num U32), Present)), (''obsv'', (TPrim (Num U32), Present))] Unboxed"
+  "abbreviatedType6 \<equiv> TRecord [(''acc'', (abbreviatedType5, Present)), (''obsv'', (TPrim (Num U64), Present))] Unboxed"
+
+definition
+  abbreviatedType7 :: " Cogent.type"
+where
+  "abbreviatedType7 \<equiv> TRecord [(''acc'', (TPrim (Num U32), Present)), (''obsv'', (TPrim (Num U32), Present))] Unboxed"
 
 lemmas abbreviated_type_defs =
+  abbreviatedType4_def
+  abbreviatedType6_def
+  abbreviatedType7_def
+  abbreviatedType1_def
   abbreviatedType3_def
   abbreviatedType5_def
-  abbreviatedType6_def
-  abbreviatedType1_def
-  abbreviatedType4_def
   abbreviatedType2_def
 
 definition
@@ -59,22 +65,22 @@ where
 definition
   repeat_0_type :: " Cogent.kind list \<times>  Cogent.type \<times>  Cogent.type"
 where
-  "repeat_0_type \<equiv> ([], (TRecord [(''n'', (TPrim (Num U64), Present)), (''stop'', (TFun abbreviatedType5 (TPrim Bool), Present)), (''step'', (TFun abbreviatedType5 abbreviatedType4, Present)), (''acc'', (abbreviatedType4, Present)), (''obsv'', (TPrim (Num U64), Present))] Unboxed, abbreviatedType4))"
+  "repeat_0_type \<equiv> ([], (TRecord [(''n'', (TPrim (Num U64), Present)), (''stop'', (TFun abbreviatedType6 (TPrim Bool), Present)), (''step'', (TFun abbreviatedType6 abbreviatedType5, Present)), (''acc'', (abbreviatedType5, Present)), (''obsv'', (TPrim (Num U64), Present))] Unboxed, abbreviatedType5))"
 
 definition
   repeat_2_type :: " Cogent.kind list \<times>  Cogent.type \<times>  Cogent.type"
 where
-  "repeat_2_type \<equiv> ([], (TRecord [(''n'', (TPrim (Num U64), Present)), (''stop'', (TFun abbreviatedType3 (TPrim Bool), Present)), (''step'', (TFun abbreviatedType3 abbreviatedType1, Present)), (''acc'', (abbreviatedType1, Present)), (''obsv'', (abbreviatedType2, Present))] Unboxed, abbreviatedType1))"
+  "repeat_2_type \<equiv> ([], (TRecord [(''n'', (TPrim (Num U64), Present)), (''stop'', (TFun abbreviatedType4 (TPrim Bool), Present)), (''step'', (TFun abbreviatedType4 abbreviatedType3, Present)), (''acc'', (abbreviatedType3, Present)), (''obsv'', (abbreviatedType2, Present))] Unboxed, abbreviatedType3))"
 
 definition
   repeat_1_type :: " Cogent.kind list \<times>  Cogent.type \<times>  Cogent.type"
 where
-  "repeat_1_type \<equiv> ([], (TRecord [(''n'', (TPrim (Num U64), Present)), (''stop'', (TFun abbreviatedType6 (TPrim Bool), Present)), (''step'', (TFun abbreviatedType6 (TPrim (Num U32)), Present)), (''acc'', (TPrim (Num U32), Present)), (''obsv'', (TPrim (Num U32), Present))] Unboxed, TPrim (Num U32)))"
+  "repeat_1_type \<equiv> ([], (TRecord [(''n'', (TPrim (Num U64), Present)), (''stop'', (TFun abbreviatedType7 (TPrim Bool), Present)), (''step'', (TFun abbreviatedType7 (TPrim (Num U32)), Present)), (''acc'', (TPrim (Num U32), Present)), (''obsv'', (TPrim (Num U32), Present))] Unboxed, TPrim (Num U32)))"
 
 definition
   expstop_type :: " Cogent.kind list \<times>  Cogent.type \<times>  Cogent.type"
 where
-  "expstop_type \<equiv> ([], (abbreviatedType6, TPrim Bool))"
+  "expstop_type \<equiv> ([], (abbreviatedType7, TPrim Bool))"
 
 definition
   expstop :: "string Cogent.expr"
@@ -84,7 +90,7 @@ where
 definition
   log2stop_type :: " Cogent.kind list \<times>  Cogent.type \<times>  Cogent.type"
 where
-  "log2stop_type \<equiv> ([], (abbreviatedType5, TPrim Bool))"
+  "log2stop_type \<equiv> ([], (abbreviatedType6, TPrim Bool))"
 
 definition
   log2stop :: "string Cogent.expr"
@@ -94,17 +100,17 @@ where
 definition
   searchStop_type :: " Cogent.kind list \<times>  Cogent.type \<times>  Cogent.type"
 where
-  "searchStop_type \<equiv> ([], (abbreviatedType3, TPrim Bool))"
+  "searchStop_type \<equiv> ([], (abbreviatedType4, TPrim Bool))"
 
 definition
   searchStop :: "string Cogent.expr"
 where
-  "searchStop \<equiv> Take (Var 0) 0 (Take (Var 1) 1 (Take (Var 2) 0 (Take (Var 1) 1 (Take (Var 4) 0 (Take (Var 1) 1 (Let (App (AFun ''wordarray_length_0'' []) (Var 2)) (Let (Lit (LU32 0)) (Let (Struct [TCon ''WordArray'' [TPrim (Num U32)] (Boxed ReadOnly undefined), TPrim (Num U32), TPrim (Num U32)] [Var 4, Var 8, Var 0]) (Let (App (AFun ''wordarray_get_0'' []) (Var 0)) (Let (Prim (Ge U32) [Var 10, Var 8]) (If (Var 0) (Lit (LBool True)) (Lit (LBool False)))))))))))))"
+  "searchStop \<equiv> Take (Var 0) 0 (Take (Var 1) 1 (Take (Var 2) 0 (Take (Var 1) 1 (Take (Var 1) 2 (If (Var 0) (Lit (LBool True)) (Let (Prim (Ge U32) [Var 4, Var 2]) (If (Var 0) (Lit (LBool True)) (Lit (LBool False)))))))))"
 
 definition
   expstep_type :: " Cogent.kind list \<times>  Cogent.type \<times>  Cogent.type"
 where
-  "expstep_type \<equiv> ([], (abbreviatedType6, TPrim (Num U32)))"
+  "expstep_type \<equiv> ([], (abbreviatedType7, TPrim (Num U32)))"
 
 definition
   expstep :: "string Cogent.expr"
@@ -114,7 +120,7 @@ where
 definition
   log2step_type :: " Cogent.kind list \<times>  Cogent.type \<times>  Cogent.type"
 where
-  "log2step_type \<equiv> ([], (abbreviatedType5, abbreviatedType4))"
+  "log2step_type \<equiv> ([], (abbreviatedType6, abbreviatedType5))"
 
 definition
   log2step :: "string Cogent.expr"
@@ -124,12 +130,12 @@ where
 definition
   searchNext_type :: " Cogent.kind list \<times>  Cogent.type \<times>  Cogent.type"
 where
-  "searchNext_type \<equiv> ([], (abbreviatedType3, abbreviatedType1))"
+  "searchNext_type \<equiv> ([], (abbreviatedType4, abbreviatedType3))"
 
 definition
   searchNext :: "string Cogent.expr"
 where
-  "searchNext \<equiv> Take (Var 0) 0 (Take (Var 1) 1 (Take (Var 2) 0 (Take (Var 1) 1 (Take (Var 4) 0 (Take (Var 1) 1 (Let (Prim (Minus U32) [Var 4, Var 6]) (Let (Lit (LU32 2)) (Let (Prim (Divide U32) [Var 1, Var 0]) (Let (Prim (Plus U32) [Var 9, Var 0]) (Let (Lit (LU32 0)) (Let (Struct [TCon ''WordArray'' [TPrim (Num U32)] (Boxed ReadOnly undefined), TPrim (Num U32), TPrim (Num U32)] [Var 7, Var 1, Var 0]) (Let (App (AFun ''wordarray_get_0'' []) (Var 0)) (Let (Prim (Lt U32) [Var 0, Var 7]) (If (Var 0) (Let (Lit (LU32 1)) (Let (Prim (Plus U32) [Var 5, Var 0]) (Struct [TPrim (Num U32), TPrim (Num U32)] [Var 0, Var 14]))) (Struct [TPrim (Num U32), TPrim (Num U32)] [Var 14, Var 4])))))))))))))))"
+  "searchNext \<equiv> Take (Var 0) 0 (Take (Var 1) 1 (Take (Var 2) 0 (Take (Var 1) 1 (Take (Var 1) 2 (Take (Var 6) 0 (Take (Var 1) 1 (Let (Prim (Minus U32) [Var 6, Var 8]) (Let (Lit (LU32 2)) (Let (Prim (Divide U32) [Var 1, Var 0]) (Let (Prim (Plus U32) [Var 11, Var 0]) (Let (Lit (LU32 0)) (Let (Struct [TCon ''WordArray'' [TPrim (Num U32)] (Boxed ReadOnly undefined), TPrim (Num U32), TPrim (Num U32)] [Var 7, Var 1, Var 0]) (Let (App (AFun ''wordarray_get_0'' []) (Var 0)) (Let (Prim (Lt U32) [Var 0, Var 7]) (If (Var 0) (Let (Lit (LU32 1)) (Let (Prim (Plus U32) [Var 5, Var 0]) (Struct [TPrim (Num U32), TPrim (Num U32), TPrim Bool] [Var 0, Var 16, Var 14]))) (Let (Prim (Gt U32) [Var 1, Var 8]) (If (Var 0) (Struct [TPrim (Num U32), TPrim (Num U32), TPrim Bool] [Var 17, Var 5, Var 13]) (Let (Lit (LBool True)) (Struct [TPrim (Num U32), TPrim (Num U32), TPrim Bool] [Var 6, Var 16, Var 0])))))))))))))))))))"
 
 definition
   binarySearch_type :: " Cogent.kind list \<times>  Cogent.type \<times>  Cogent.type"
@@ -139,7 +145,7 @@ where
 definition
   binarySearch :: "string Cogent.expr"
 where
-  "binarySearch \<equiv> Take (Var 0) 0 (Take (Var 1) 1 (Let (App (AFun ''wordarray_length_0'' []) (Var 2)) (Let (Cast U64 (Var 0)) (Let (Fun searchStop []) (Let (Fun searchNext []) (Let (Lit (LU32 0)) (Let (Struct [TPrim (Num U32), TPrim (Num U32)] [Var 0, Var 4]) (Let (Struct [TCon ''WordArray'' [TPrim (Num U32)] (Boxed ReadOnly undefined), TPrim (Num U32)] [Var 8, Var 6]) (Let (Struct [TPrim (Num U64), TFun abbreviatedType3 (TPrim Bool), TFun abbreviatedType3 abbreviatedType1, abbreviatedType1, abbreviatedType2] [Var 5, Var 4, Var 3, Var 1, Var 0]) (Let (App (AFun ''repeat_2'' []) (Var 0)) (Take (Var 0) 0 (Take (Var 1) 1 (Var 2)))))))))))))"
+  "binarySearch \<equiv> Take (Var 0) 0 (Take (Var 1) 1 (Let (App (AFun ''wordarray_length_0'' []) (Var 2)) (Let (Cast U64 (Var 0)) (Let (Fun searchStop []) (Let (Fun searchNext []) (Let (Lit (LU32 0)) (Let (Lit (LBool False)) (Let (Struct [TPrim (Num U32), TPrim (Num U32), TPrim Bool] [Var 1, Var 5, Var 0]) (Let (Struct [TCon ''WordArray'' [TPrim (Num U32)] (Boxed ReadOnly undefined), TPrim (Num U32)] [Var 9, Var 7]) (Let (Struct [TPrim (Num U64), TFun abbreviatedType4 (TPrim Bool), TFun abbreviatedType4 abbreviatedType3, abbreviatedType3, abbreviatedType2] [Var 6, Var 5, Var 4, Var 1, Var 0]) (Let (App (AFun ''repeat_2'' []) (Var 0)) (Take (Var 0) 0 (Take (Var 1) 1 (Take (Var 1) 2 (If (Var 0) (Var 4) (Var 15))))))))))))))))"
 
 definition
   myexp_type :: " Cogent.kind list \<times>  Cogent.type \<times>  Cogent.type"
@@ -149,7 +155,7 @@ where
 definition
   myexp :: "string Cogent.expr"
 where
-  "myexp \<equiv> Take (Var 0) 0 (Take (Var 1) 1 (Let (Cast U64 (Var 0)) (Let (Fun expstop []) (Let (Fun expstep []) (Let (Lit (LU32 1)) (Let (Struct [TPrim (Num U64), TFun abbreviatedType6 (TPrim Bool), TFun abbreviatedType6 (TPrim (Num U32)), TPrim (Num U32), TPrim (Num U32)] [Var 3, Var 2, Var 1, Var 0, Var 6]) (App (AFun ''repeat_1'' []) (Var 0))))))))"
+  "myexp \<equiv> Take (Var 0) 0 (Take (Var 1) 1 (Let (Cast U64 (Var 0)) (Let (Fun expstop []) (Let (Fun expstep []) (Let (Lit (LU32 1)) (Let (Struct [TPrim (Num U64), TFun abbreviatedType7 (TPrim Bool), TFun abbreviatedType7 (TPrim (Num U32)), TPrim (Num U32), TPrim (Num U32)] [Var 3, Var 2, Var 1, Var 0, Var 6]) (App (AFun ''repeat_1'' []) (Var 0))))))))"
 
 definition
   mylog2_type :: " Cogent.kind list \<times>  Cogent.type \<times>  Cogent.type"
@@ -159,7 +165,7 @@ where
 definition
   mylog2 :: "string Cogent.expr"
 where
-  "mylog2 \<equiv> Let (Var 0) (Let (Fun log2stop []) (Let (Fun log2step []) (Let (Lit (LU64 1)) (Let (Lit (LU64 0)) (Let (Struct [TPrim (Num U64), TPrim (Num U64)] [Var 1, Var 0]) (Let (Struct [TPrim (Num U64), TFun abbreviatedType5 (TPrim Bool), TFun abbreviatedType5 abbreviatedType4, abbreviatedType4, TPrim (Num U64)] [Var 5, Var 4, Var 3, Var 0, Var 5]) (Let (App (AFun ''repeat_0'' []) (Var 0)) (Take (Var 0) 0 (Take (Var 1) 1 (Var 0))))))))))"
+  "mylog2 \<equiv> Let (Var 0) (Let (Fun log2stop []) (Let (Fun log2step []) (Let (Lit (LU64 1)) (Let (Lit (LU64 0)) (Let (Struct [TPrim (Num U64), TPrim (Num U64)] [Var 1, Var 0]) (Let (Struct [TPrim (Num U64), TFun abbreviatedType6 (TPrim Bool), TFun abbreviatedType6 abbreviatedType5, abbreviatedType5, TPrim (Num U64)] [Var 5, Var 4, Var 3, Var 0, Var 5]) (Let (App (AFun ''repeat_0'' []) (Var 0)) (Take (Var 0) 0 (Take (Var 1) 1 (Var 0))))))))))"
 
 ML \<open>
 val Cogent_functions = ["expstop", "log2stop", "searchStop", "expstep", "log2step", "searchNext", "binarySearch", "myexp", "mylog2"]
@@ -175,31 +181,31 @@ definition
   "\<xi> \<equiv> assoc_lookup [(''wordarray_get_0'', (\<lambda>_ _. False)), (''wordarray_length_0'', (\<lambda>_ _. False)), (''repeat_0'', (\<lambda>_ _. False)), (''repeat_2'', (\<lambda>_ _. False)), (''repeat_1'', (\<lambda>_ _. False))]"
 
 definition
-  "expstop_typetree \<equiv> TyTrSplit (Cons (Some TSK_L) []) [] TyTrLeaf [Some abbreviatedType6] TyTrLeaf"
+  "expstop_typetree \<equiv> TyTrSplit (Cons (Some TSK_L) []) [] TyTrLeaf [Some abbreviatedType7] TyTrLeaf"
 
 definition
-  "log2stop_typetree \<equiv> TyTrSplit (Cons (Some TSK_L) []) [] TyTrLeaf [Some abbreviatedType4, Some (TRecord [(''acc'', (abbreviatedType4, Taken)), (''obsv'', (TPrim (Num U64), Present))] Unboxed)] (TyTrSplit (Cons (Some TSK_R) (Cons (Some TSK_L) (Cons None []))) [] TyTrLeaf [Some (TPrim (Num U64)), Some (TRecord [(''acc'', (abbreviatedType4, Taken)), (''obsv'', (TPrim (Num U64), Taken))] Unboxed)] (TyTrSplit (Cons (Some TSK_R) (Cons (Some TSK_L) (Cons (Some TSK_L) (append (replicate 2 None) [])))) [] TyTrLeaf [Some (TPrim (Num U64)), Some (TRecord [(''p1'', (TPrim (Num U64), Taken)), (''p2'', (TPrim (Num U64), Present))] Unboxed)] (TyTrSplit (Cons (Some TSK_R) (Cons (Some TSK_L) (Cons (Some TSK_R) (append (replicate 4 None) [])))) [] TyTrLeaf [Some (TPrim (Num U64)), Some (TRecord [(''p1'', (TPrim (Num U64), Taken)), (''p2'', (TPrim (Num U64), Taken))] Unboxed)] TyTrLeaf)))"
+  "log2stop_typetree \<equiv> TyTrSplit (Cons (Some TSK_L) []) [] TyTrLeaf [Some abbreviatedType5, Some (TRecord [(''acc'', (abbreviatedType5, Taken)), (''obsv'', (TPrim (Num U64), Present))] Unboxed)] (TyTrSplit (Cons (Some TSK_R) (Cons (Some TSK_L) (Cons None []))) [] TyTrLeaf [Some (TPrim (Num U64)), Some (TRecord [(''acc'', (abbreviatedType5, Taken)), (''obsv'', (TPrim (Num U64), Taken))] Unboxed)] (TyTrSplit (Cons (Some TSK_R) (Cons (Some TSK_L) (Cons (Some TSK_L) (append (replicate 2 None) [])))) [] TyTrLeaf [Some (TPrim (Num U64)), Some (TRecord [(''p1'', (TPrim (Num U64), Taken)), (''p2'', (TPrim (Num U64), Present))] Unboxed)] (TyTrSplit (Cons (Some TSK_R) (Cons (Some TSK_L) (Cons (Some TSK_R) (append (replicate 4 None) [])))) [] TyTrLeaf [Some (TPrim (Num U64)), Some (TRecord [(''p1'', (TPrim (Num U64), Taken)), (''p2'', (TPrim (Num U64), Taken))] Unboxed)] TyTrLeaf)))"
 
 definition
-  "searchStop_typetree \<equiv> TyTrSplit (Cons (Some TSK_L) []) [] TyTrLeaf [Some abbreviatedType1, Some (TRecord [(''acc'', (abbreviatedType1, Taken)), (''obsv'', (abbreviatedType2, Present))] Unboxed)] (TyTrSplit (Cons (Some TSK_R) (Cons (Some TSK_L) (Cons None []))) [] TyTrLeaf [Some abbreviatedType2, Some (TRecord [(''acc'', (abbreviatedType1, Taken)), (''obsv'', (abbreviatedType2, Taken))] Unboxed)] (TyTrSplit (Cons (Some TSK_R) (Cons (Some TSK_L) (Cons (Some TSK_L) (append (replicate 2 None) [])))) [] TyTrLeaf [Some (TPrim (Num U32)), Some (TRecord [(''p1'', (TPrim (Num U32), Taken)), (''p2'', (TPrim (Num U32), Present))] Unboxed)] (TyTrSplit (Cons (Some TSK_R) (Cons (Some TSK_L) (Cons (Some TSK_R) (append (replicate 4 None) [])))) [] TyTrLeaf [Some (TPrim (Num U32)), Some (TRecord [(''p1'', (TPrim (Num U32), Taken)), (''p2'', (TPrim (Num U32), Taken))] Unboxed)] (TyTrSplit (Cons (Some TSK_R) (Cons (Some TSK_L) (Cons (Some TSK_R) (Cons None (Cons (Some TSK_L) (append (replicate 4 None) [])))))) [] TyTrLeaf [Some (TCon ''WordArray'' [TPrim (Num U32)] (Boxed ReadOnly undefined)), Some (TRecord [(''p1'', (TCon ''WordArray'' [TPrim (Num U32)] (Boxed ReadOnly undefined), Taken)), (''p2'', (TPrim (Num U32), Present))] Unboxed)] (TyTrSplit (Cons (Some TSK_R) (Cons (Some TSK_L) (Cons (Some TSK_R) (Cons None (Cons (Some TSK_R) (append (replicate 6 None) [])))))) [] TyTrLeaf [Some (TPrim (Num U32)), Some (TRecord [(''p1'', (TCon ''WordArray'' [TPrim (Num U32)] (Boxed ReadOnly undefined), Taken)), (''p2'', (TPrim (Num U32), Taken))] Unboxed)] (TyTrSplit (Cons (Some TSK_L) (Cons (Some TSK_L) (Cons (Some TSK_S) (Cons None (Cons (Some TSK_R) (Cons None (Cons (Some TSK_R) (append (replicate 6 None) [])))))))) [] TyTrLeaf [Some (TPrim (Num U32))] (TyTrSplit (Cons (Some TSK_L) (append (replicate 2 None) (Cons (Some TSK_R) (Cons None (Cons (Some TSK_R) (Cons None (Cons (Some TSK_R) (append (replicate 6 None) [])))))))) [] TyTrLeaf [Some (TPrim (Num U32))] (TyTrSplit (Cons (Some TSK_L) (append (replicate 3 None) (Cons (Some TSK_L) (Cons None (Cons (Some TSK_R) (Cons None (Cons (Some TSK_S) (append (replicate 6 None) [])))))))) [] TyTrLeaf [Some (TRecord [(''arr'', (TCon ''WordArray'' [TPrim (Num U32)] (Boxed ReadOnly undefined), Present)), (''idx'', (TPrim (Num U32), Present)), (''val'', (TPrim (Num U32), Present))] Unboxed)] (TyTrSplit (Cons (Some TSK_L) (append (replicate 6 None) (Cons (Some TSK_R) (Cons None (Cons (Some TSK_R) (append (replicate 6 None) [])))))) [] TyTrLeaf [Some (TPrim (Num U32))] (TyTrSplit (Cons (Some TSK_L) (append (replicate 7 None) (Cons (Some TSK_L) (Cons None (Cons (Some TSK_L) (append (replicate 6 None) [])))))) [] TyTrLeaf [Some (TPrim Bool)] (TyTrSplit (Cons (Some TSK_L) (append (replicate 17 None) [])) [] TyTrLeaf [] (TyTrSplit (append (replicate 18 None) []) [] TyTrLeaf [] TyTrLeaf))))))))))))"
+  "searchStop_typetree \<equiv> TyTrSplit (Cons (Some TSK_L) []) [] TyTrLeaf [Some abbreviatedType3, Some (TRecord [(''acc'', (abbreviatedType3, Taken)), (''obsv'', (abbreviatedType2, Present))] Unboxed)] (TyTrSplit (Cons (Some TSK_R) (Cons (Some TSK_L) (Cons None []))) [] TyTrLeaf [Some abbreviatedType2, Some (TRecord [(''acc'', (abbreviatedType3, Taken)), (''obsv'', (abbreviatedType2, Taken))] Unboxed)] (TyTrSplit (Cons (Some TSK_L) (Cons (Some TSK_L) (Cons (Some TSK_L) (append (replicate 2 None) [])))) [] TyTrLeaf [Some (TPrim (Num U32)), Some (TRecord [(''p1'', (TPrim (Num U32), Taken)), (''p2'', (TPrim (Num U32), Present)), (''p3'', (TPrim Bool, Present))] Unboxed)] (TyTrSplit (Cons (Some TSK_R) (Cons (Some TSK_L) (append (replicate 5 None) []))) [] TyTrLeaf [Some (TPrim (Num U32)), Some (TRecord [(''p1'', (TPrim (Num U32), Taken)), (''p2'', (TPrim (Num U32), Taken)), (''p3'', (TPrim Bool, Present))] Unboxed)] (TyTrSplit (Cons (Some TSK_R) (Cons (Some TSK_L) (Cons (Some TSK_R) (append (replicate 6 None) [])))) [] TyTrLeaf [Some (TPrim Bool), Some (TRecord [(''p1'', (TPrim (Num U32), Taken)), (''p2'', (TPrim (Num U32), Taken)), (''p3'', (TPrim Bool, Taken))] Unboxed)] (TyTrSplit (Cons (Some TSK_L) (Cons (Some TSK_L) (Cons (Some TSK_R) (Cons None (Cons (Some TSK_R) (append (replicate 6 None) [])))))) [] TyTrLeaf [] (TyTrSplit (append (replicate 2 None) (Cons (Some TSK_S) (Cons None (Cons (Some TSK_S) (append (replicate 6 None) []))))) [] TyTrLeaf [] (TyTrSplit (append (replicate 2 None) (Cons (Some TSK_L) (Cons None (Cons (Some TSK_L) (append (replicate 6 None) []))))) [] TyTrLeaf [Some (TPrim Bool)] (TyTrSplit (Cons (Some TSK_L) (append (replicate 11 None) [])) [] TyTrLeaf [] (TyTrSplit (append (replicate 12 None) []) [] TyTrLeaf [] TyTrLeaf)))))))))"
 
 definition
   "expstep_typetree \<equiv> TyTrSplit (Cons (Some TSK_L) []) [] TyTrLeaf [Some (TPrim (Num U32)), Some (TRecord [(''acc'', (TPrim (Num U32), Taken)), (''obsv'', (TPrim (Num U32), Present))] Unboxed)] (TyTrSplit (Cons (Some TSK_R) (Cons (Some TSK_L) (Cons None []))) [] TyTrLeaf [Some (TPrim (Num U32)), Some (TRecord [(''acc'', (TPrim (Num U32), Taken)), (''obsv'', (TPrim (Num U32), Taken))] Unboxed)] TyTrLeaf)"
 
 definition
-  "log2step_typetree \<equiv> TyTrSplit (Cons (Some TSK_L) []) [] TyTrLeaf [Some abbreviatedType4, Some (TRecord [(''acc'', (abbreviatedType4, Taken)), (''obsv'', (TPrim (Num U64), Present))] Unboxed)] (TyTrSplit (Cons (Some TSK_R) (Cons (Some TSK_L) (Cons None []))) [] TyTrLeaf [Some (TPrim (Num U64)), Some (TRecord [(''acc'', (abbreviatedType4, Taken)), (''obsv'', (TPrim (Num U64), Taken))] Unboxed)] (TyTrSplit (Cons (Some TSK_L) (Cons (Some TSK_L) (Cons (Some TSK_L) (append (replicate 2 None) [])))) [] TyTrLeaf [Some (TPrim (Num U64)), Some (TRecord [(''p1'', (TPrim (Num U64), Taken)), (''p2'', (TPrim (Num U64), Present))] Unboxed)] (TyTrSplit (Cons (Some TSK_R) (Cons (Some TSK_L) (append (replicate 5 None) []))) [] TyTrLeaf [Some (TPrim (Num U64)), Some (TRecord [(''p1'', (TPrim (Num U64), Taken)), (''p2'', (TPrim (Num U64), Taken))] Unboxed)] (TyTrSplit (Cons (Some TSK_R) (Cons (Some TSK_L) (Cons (Some TSK_R) (append (replicate 6 None) [])))) [] TyTrLeaf [Some (TPrim (Num U64))] (TyTrSplit (Cons (Some TSK_L) (Cons (Some TSK_R) (Cons None (Cons (Some TSK_L) (append (replicate 6 None) []))))) [] TyTrLeaf [Some (TPrim (Num U64))] (TyTrSplit (Cons (Some TSK_R) (Cons None (Cons (Some TSK_R) (append (replicate 8 None) [])))) [] TyTrLeaf [Some (TPrim (Num U64))] (TyTrSplit (Cons (Some TSK_L) (Cons (Some TSK_R) (Cons None (Cons (Some TSK_L) (append (replicate 8 None) []))))) [] TyTrLeaf [Some (TPrim (Num U64))] TyTrLeaf)))))))"
+  "log2step_typetree \<equiv> TyTrSplit (Cons (Some TSK_L) []) [] TyTrLeaf [Some abbreviatedType5, Some (TRecord [(''acc'', (abbreviatedType5, Taken)), (''obsv'', (TPrim (Num U64), Present))] Unboxed)] (TyTrSplit (Cons (Some TSK_R) (Cons (Some TSK_L) (Cons None []))) [] TyTrLeaf [Some (TPrim (Num U64)), Some (TRecord [(''acc'', (abbreviatedType5, Taken)), (''obsv'', (TPrim (Num U64), Taken))] Unboxed)] (TyTrSplit (Cons (Some TSK_L) (Cons (Some TSK_L) (Cons (Some TSK_L) (append (replicate 2 None) [])))) [] TyTrLeaf [Some (TPrim (Num U64)), Some (TRecord [(''p1'', (TPrim (Num U64), Taken)), (''p2'', (TPrim (Num U64), Present))] Unboxed)] (TyTrSplit (Cons (Some TSK_R) (Cons (Some TSK_L) (append (replicate 5 None) []))) [] TyTrLeaf [Some (TPrim (Num U64)), Some (TRecord [(''p1'', (TPrim (Num U64), Taken)), (''p2'', (TPrim (Num U64), Taken))] Unboxed)] (TyTrSplit (Cons (Some TSK_R) (Cons (Some TSK_L) (Cons (Some TSK_R) (append (replicate 6 None) [])))) [] TyTrLeaf [Some (TPrim (Num U64))] (TyTrSplit (Cons (Some TSK_L) (Cons (Some TSK_R) (Cons None (Cons (Some TSK_L) (append (replicate 6 None) []))))) [] TyTrLeaf [Some (TPrim (Num U64))] (TyTrSplit (Cons (Some TSK_R) (Cons None (Cons (Some TSK_R) (append (replicate 8 None) [])))) [] TyTrLeaf [Some (TPrim (Num U64))] (TyTrSplit (Cons (Some TSK_L) (Cons (Some TSK_R) (Cons None (Cons (Some TSK_L) (append (replicate 8 None) []))))) [] TyTrLeaf [Some (TPrim (Num U64))] TyTrLeaf)))))))"
 
 definition
-  "searchNext_typetree \<equiv> TyTrSplit (Cons (Some TSK_L) []) [] TyTrLeaf [Some abbreviatedType1, Some (TRecord [(''acc'', (abbreviatedType1, Taken)), (''obsv'', (abbreviatedType2, Present))] Unboxed)] (TyTrSplit (Cons (Some TSK_R) (Cons (Some TSK_L) (Cons None []))) [] TyTrLeaf [Some abbreviatedType2, Some (TRecord [(''acc'', (abbreviatedType1, Taken)), (''obsv'', (abbreviatedType2, Taken))] Unboxed)] (TyTrSplit (Cons (Some TSK_R) (Cons (Some TSK_L) (Cons (Some TSK_L) (append (replicate 2 None) [])))) [] TyTrLeaf [Some (TPrim (Num U32)), Some (TRecord [(''p1'', (TPrim (Num U32), Taken)), (''p2'', (TPrim (Num U32), Present))] Unboxed)] (TyTrSplit (Cons (Some TSK_R) (Cons (Some TSK_L) (Cons (Some TSK_R) (append (replicate 4 None) [])))) [] TyTrLeaf [Some (TPrim (Num U32)), Some (TRecord [(''p1'', (TPrim (Num U32), Taken)), (''p2'', (TPrim (Num U32), Taken))] Unboxed)] (TyTrSplit (Cons (Some TSK_R) (Cons (Some TSK_L) (Cons (Some TSK_R) (Cons None (Cons (Some TSK_L) (append (replicate 4 None) [])))))) [] TyTrLeaf [Some (TCon ''WordArray'' [TPrim (Num U32)] (Boxed ReadOnly undefined)), Some (TRecord [(''p1'', (TCon ''WordArray'' [TPrim (Num U32)] (Boxed ReadOnly undefined), Taken)), (''p2'', (TPrim (Num U32), Present))] Unboxed)] (TyTrSplit (Cons (Some TSK_R) (Cons (Some TSK_L) (Cons (Some TSK_R) (Cons None (Cons (Some TSK_R) (append (replicate 6 None) [])))))) [] TyTrLeaf [Some (TPrim (Num U32)), Some (TRecord [(''p1'', (TCon ''WordArray'' [TPrim (Num U32)] (Boxed ReadOnly undefined), Taken)), (''p2'', (TPrim (Num U32), Taken))] Unboxed)] (TyTrSplit (Cons (Some TSK_R) (Cons (Some TSK_L) (Cons (Some TSK_R) (Cons None (Cons (Some TSK_S) (Cons None (Cons (Some TSK_S) (append (replicate 6 None) [])))))))) [] TyTrLeaf [Some (TPrim (Num U32))] (TyTrSplit (Cons (Some TSK_R) (Cons (Some TSK_R) (Cons None (Cons (Some TSK_R) (Cons None (Cons (Some TSK_R) (Cons None (Cons (Some TSK_R) (append (replicate 6 None) []))))))))) [] TyTrLeaf [Some (TPrim (Num U32))] (TyTrSplit (Cons (Some TSK_L) (Cons (Some TSK_L) (Cons (Some TSK_R) (Cons None (Cons (Some TSK_R) (Cons None (Cons (Some TSK_R) (Cons None (Cons (Some TSK_R) (append (replicate 6 None) [])))))))))) [] TyTrLeaf [Some (TPrim (Num U32))] (TyTrSplit (Cons (Some TSK_L) (append (replicate 2 None) (Cons (Some TSK_R) (Cons None (Cons (Some TSK_R) (Cons None (Cons (Some TSK_R) (Cons None (Cons (Some TSK_S) (append (replicate 6 None) [])))))))))) [] TyTrLeaf [Some (TPrim (Num U32))] (TyTrSplit (Cons (Some TSK_R) (append (replicate 3 None) (Cons (Some TSK_R) (Cons None (Cons (Some TSK_R) (Cons None (Cons (Some TSK_R) (Cons None (Cons (Some TSK_R) (append (replicate 6 None) [])))))))))) [] TyTrLeaf [Some (TPrim (Num U32))] (TyTrSplit (Cons (Some TSK_L) (Cons (Some TSK_S) (append (replicate 3 None) (Cons (Some TSK_R) (Cons None (Cons (Some TSK_L) (Cons None (Cons (Some TSK_R) (Cons None (Cons (Some TSK_R) (append (replicate 6 None) []))))))))))) [] TyTrLeaf [Some (TRecord [(''arr'', (TCon ''WordArray'' [TPrim (Num U32)] (Boxed ReadOnly undefined), Present)), (''idx'', (TPrim (Num U32), Present)), (''val'', (TPrim (Num U32), Present))] Unboxed)] (TyTrSplit (Cons (Some TSK_L) (Cons None (Cons (Some TSK_R) (append (replicate 3 None) (Cons (Some TSK_R) (append (replicate 3 None) (Cons (Some TSK_R) (Cons None (Cons (Some TSK_R) (append (replicate 6 None) [])))))))))) [] TyTrLeaf [Some (TPrim (Num U32))] (TyTrSplit (Cons (Some TSK_L) (append (replicate 2 None) (Cons (Some TSK_R) (append (replicate 3 None) (Cons (Some TSK_L) (append (replicate 3 None) (Cons (Some TSK_R) (Cons None (Cons (Some TSK_R) (append (replicate 6 None) [])))))))))) [] TyTrLeaf [Some (TPrim Bool)] (TyTrSplit (Cons (Some TSK_L) (append (replicate 3 None) (Cons (Some TSK_R) (append (replicate 7 None) (Cons (Some TSK_R) (Cons None (Cons (Some TSK_R) (append (replicate 6 None) [])))))))) [] TyTrLeaf [] (TyTrSplit (append (replicate 4 None) (Cons (Some TSK_S) (append (replicate 7 None) (Cons (Some TSK_S) (Cons None (Cons (Some TSK_S) (append (replicate 6 None) []))))))) [] (TyTrSplit (append (replicate 4 None) (Cons (Some TSK_R) (append (replicate 7 None) (Cons (Some TSK_R) (Cons None (Cons (Some TSK_L) (append (replicate 6 None) []))))))) [] TyTrLeaf [Some (TPrim (Num U32))] (TyTrSplit (Cons (Some TSK_L) (append (replicate 4 None) (Cons (Some TSK_L) (append (replicate 7 None) (Cons (Some TSK_R) (append (replicate 8 None) [])))))) [] TyTrLeaf [Some (TPrim (Num U32))] TyTrLeaf)) [] TyTrLeaf)))))))))))))))"
+  "searchNext_typetree \<equiv> TyTrSplit (Cons (Some TSK_L) []) [] TyTrLeaf [Some abbreviatedType3, Some (TRecord [(''acc'', (abbreviatedType3, Taken)), (''obsv'', (abbreviatedType2, Present))] Unboxed)] (TyTrSplit (Cons (Some TSK_R) (Cons (Some TSK_L) (Cons None []))) [] TyTrLeaf [Some abbreviatedType2, Some (TRecord [(''acc'', (abbreviatedType3, Taken)), (''obsv'', (abbreviatedType2, Taken))] Unboxed)] (TyTrSplit (Cons (Some TSK_R) (Cons (Some TSK_L) (Cons (Some TSK_L) (append (replicate 2 None) [])))) [] TyTrLeaf [Some (TPrim (Num U32)), Some (TRecord [(''p1'', (TPrim (Num U32), Taken)), (''p2'', (TPrim (Num U32), Present)), (''p3'', (TPrim Bool, Present))] Unboxed)] (TyTrSplit (Cons (Some TSK_R) (Cons (Some TSK_L) (Cons (Some TSK_R) (append (replicate 4 None) [])))) [] TyTrLeaf [Some (TPrim (Num U32)), Some (TRecord [(''p1'', (TPrim (Num U32), Taken)), (''p2'', (TPrim (Num U32), Taken)), (''p3'', (TPrim Bool, Present))] Unboxed)] (TyTrSplit (Cons (Some TSK_R) (Cons (Some TSK_L) (Cons (Some TSK_R) (Cons None (Cons (Some TSK_R) (append (replicate 4 None) [])))))) [] TyTrLeaf [Some (TPrim Bool), Some (TRecord [(''p1'', (TPrim (Num U32), Taken)), (''p2'', (TPrim (Num U32), Taken)), (''p3'', (TPrim Bool, Taken))] Unboxed)] (TyTrSplit (Cons (Some TSK_R) (Cons (Some TSK_L) (Cons (Some TSK_R) (Cons None (Cons (Some TSK_R) (Cons None (Cons (Some TSK_L) (append (replicate 4 None) [])))))))) [] TyTrLeaf [Some (TCon ''WordArray'' [TPrim (Num U32)] (Boxed ReadOnly undefined)), Some (TRecord [(''p1'', (TCon ''WordArray'' [TPrim (Num U32)] (Boxed ReadOnly undefined), Taken)), (''p2'', (TPrim (Num U32), Present))] Unboxed)] (TyTrSplit (Cons (Some TSK_R) (Cons (Some TSK_L) (Cons (Some TSK_R) (Cons None (Cons (Some TSK_R) (Cons None (Cons (Some TSK_R) (append (replicate 6 None) [])))))))) [] TyTrLeaf [Some (TPrim (Num U32)), Some (TRecord [(''p1'', (TCon ''WordArray'' [TPrim (Num U32)] (Boxed ReadOnly undefined), Taken)), (''p2'', (TPrim (Num U32), Taken))] Unboxed)] (TyTrSplit (Cons (Some TSK_R) (Cons (Some TSK_L) (Cons (Some TSK_R) (Cons None (Cons (Some TSK_R) (Cons None (Cons (Some TSK_S) (Cons None (Cons (Some TSK_S) (append (replicate 6 None) [])))))))))) [] TyTrLeaf [Some (TPrim (Num U32))] (TyTrSplit (Cons (Some TSK_R) (Cons (Some TSK_R) (Cons None (Cons (Some TSK_R) (Cons None (Cons (Some TSK_R) (Cons None (Cons (Some TSK_R) (Cons None (Cons (Some TSK_R) (append (replicate 6 None) []))))))))))) [] TyTrLeaf [Some (TPrim (Num U32))] (TyTrSplit (Cons (Some TSK_L) (Cons (Some TSK_L) (Cons (Some TSK_R) (Cons None (Cons (Some TSK_R) (Cons None (Cons (Some TSK_R) (Cons None (Cons (Some TSK_R) (Cons None (Cons (Some TSK_R) (append (replicate 6 None) [])))))))))))) [] TyTrLeaf [Some (TPrim (Num U32))] (TyTrSplit (Cons (Some TSK_L) (append (replicate 2 None) (Cons (Some TSK_R) (Cons None (Cons (Some TSK_R) (Cons None (Cons (Some TSK_R) (Cons None (Cons (Some TSK_R) (Cons None (Cons (Some TSK_S) (append (replicate 6 None) [])))))))))))) [] TyTrLeaf [Some (TPrim (Num U32))] (TyTrSplit (Cons (Some TSK_R) (append (replicate 3 None) (Cons (Some TSK_R) (Cons None (Cons (Some TSK_R) (Cons None (Cons (Some TSK_R) (Cons None (Cons (Some TSK_R) (Cons None (Cons (Some TSK_R) (append (replicate 6 None) [])))))))))))) [] TyTrLeaf [Some (TPrim (Num U32))] (TyTrSplit (Cons (Some TSK_L) (Cons (Some TSK_S) (append (replicate 3 None) (Cons (Some TSK_R) (Cons None (Cons (Some TSK_L) (Cons None (Cons (Some TSK_R) (Cons None (Cons (Some TSK_R) (Cons None (Cons (Some TSK_R) (append (replicate 6 None) []))))))))))))) [] TyTrLeaf [Some (TRecord [(''arr'', (TCon ''WordArray'' [TPrim (Num U32)] (Boxed ReadOnly undefined), Present)), (''idx'', (TPrim (Num U32), Present)), (''val'', (TPrim (Num U32), Present))] Unboxed)] (TyTrSplit (Cons (Some TSK_L) (Cons None (Cons (Some TSK_R) (append (replicate 3 None) (Cons (Some TSK_R) (append (replicate 3 None) (Cons (Some TSK_R) (Cons None (Cons (Some TSK_R) (Cons None (Cons (Some TSK_R) (append (replicate 6 None) [])))))))))))) [] TyTrLeaf [Some (TPrim (Num U32))] (TyTrSplit (Cons (Some TSK_S) (append (replicate 2 None) (Cons (Some TSK_R) (append (replicate 3 None) (Cons (Some TSK_S) (append (replicate 3 None) (Cons (Some TSK_R) (Cons None (Cons (Some TSK_R) (Cons None (Cons (Some TSK_R) (append (replicate 6 None) [])))))))))))) [] TyTrLeaf [Some (TPrim Bool)] (TyTrSplit (Cons (Some TSK_L) (Cons (Some TSK_R) (append (replicate 2 None) (Cons (Some TSK_R) (append (replicate 3 None) (Cons (Some TSK_R) (append (replicate 3 None) (Cons (Some TSK_R) (Cons None (Cons (Some TSK_R) (Cons None (Cons (Some TSK_R) (append (replicate 6 None) []))))))))))))) [] TyTrLeaf [] (TyTrSplit (Cons None (Cons (Some TSK_S) (append (replicate 2 None) (Cons (Some TSK_S) (append (replicate 3 None) (Cons (Some TSK_S) (append (replicate 3 None) (Cons (Some TSK_S) (Cons None (Cons (Some TSK_S) (Cons None (Cons (Some TSK_S) (append (replicate 6 None) []))))))))))))) [] (TyTrSplit (Cons None (Cons (Some TSK_L) (append (replicate 2 None) (Cons (Some TSK_R) (append (replicate 3 None) (Cons (Some TSK_L) (append (replicate 3 None) (Cons (Some TSK_R) (Cons None (Cons (Some TSK_R) (Cons None (Cons (Some TSK_L) (append (replicate 6 None) []))))))))))))) [] TyTrLeaf [Some (TPrim (Num U32))] (TyTrSplit (Cons (Some TSK_L) (append (replicate 4 None) (Cons (Some TSK_L) (append (replicate 7 None) (Cons (Some TSK_R) (Cons None (Cons (Some TSK_R) (append (replicate 8 None) [])))))))) [] TyTrLeaf [Some (TPrim (Num U32))] TyTrLeaf)) [] (TyTrSplit (Cons None (Cons (Some TSK_L) (append (replicate 2 None) (Cons (Some TSK_R) (append (replicate 3 None) (Cons (Some TSK_L) (append (replicate 3 None) (Cons (Some TSK_R) (Cons None (Cons (Some TSK_R) (Cons None (Cons (Some TSK_R) (append (replicate 6 None) []))))))))))))) [] TyTrLeaf [Some (TPrim Bool)] (TyTrSplit (Cons (Some TSK_L) (append (replicate 4 None) (Cons (Some TSK_R) (append (replicate 7 None) (Cons (Some TSK_R) (Cons None (Cons (Some TSK_R) (Cons None (Cons (Some TSK_R) (append (replicate 6 None) [])))))))))) [] TyTrLeaf [] (TyTrSplit (append (replicate 5 None) (Cons (Some TSK_S) (append (replicate 7 None) (Cons (Some TSK_S) (Cons None (Cons (Some TSK_S) (Cons None (Cons (Some TSK_S) (append (replicate 6 None) []))))))))) [] TyTrLeaf [] (TyTrSplit (append (replicate 5 None) (Cons (Some TSK_R) (append (replicate 7 None) (Cons (Some TSK_L) (Cons None (Cons (Some TSK_R) (Cons None (Cons (Some TSK_L) (append (replicate 6 None) []))))))))) [] TyTrLeaf [Some (TPrim Bool)] TyTrLeaf))))))))))))))))))))"
 
 definition
-  "binarySearch_typetree \<equiv> TyTrSplit (Cons (Some TSK_L) []) [] TyTrLeaf [Some (TCon ''WordArray'' [TPrim (Num U32)] (Boxed ReadOnly undefined)), Some (TRecord [(''p1'', (TCon ''WordArray'' [TPrim (Num U32)] (Boxed ReadOnly undefined), Taken)), (''p2'', (TPrim (Num U32), Present))] Unboxed)] (TyTrSplit (Cons (Some TSK_R) (Cons (Some TSK_L) (Cons None []))) [] TyTrLeaf [Some (TPrim (Num U32)), Some (TRecord [(''p1'', (TCon ''WordArray'' [TPrim (Num U32)] (Boxed ReadOnly undefined), Taken)), (''p2'', (TPrim (Num U32), Taken))] Unboxed)] (TyTrSplit (Cons (Some TSK_R) (Cons (Some TSK_L) (Cons (Some TSK_S) (append (replicate 2 None) [])))) [] TyTrLeaf [Some (TPrim (Num U32))] (TyTrSplit (Cons (Some TSK_S) (Cons (Some TSK_R) (Cons None (Cons (Some TSK_R) (append (replicate 2 None) []))))) [] TyTrLeaf [Some (TPrim (Num U64))] (TyTrSplit (Cons (Some TSK_R) (Cons (Some TSK_R) (Cons (Some TSK_R) (Cons None (Cons (Some TSK_R) (append (replicate 2 None) [])))))) [] TyTrLeaf [Some (TFun abbreviatedType3 (TPrim Bool))] (TyTrSplit (Cons (Some TSK_R) (Cons (Some TSK_R) (Cons (Some TSK_R) (Cons (Some TSK_R) (Cons None (Cons (Some TSK_R) (append (replicate 2 None) []))))))) [] TyTrLeaf [Some (TFun abbreviatedType3 abbreviatedType1)] (TyTrSplit (Cons (Some TSK_R) (Cons (Some TSK_R) (Cons (Some TSK_R) (Cons (Some TSK_R) (Cons (Some TSK_R) (Cons None (Cons (Some TSK_R) (append (replicate 2 None) [])))))))) [] TyTrLeaf [Some (TPrim (Num U32))] (TyTrSplit (Cons (Some TSK_L) (Cons (Some TSK_R) (Cons (Some TSK_R) (Cons (Some TSK_R) (Cons (Some TSK_L) (Cons (Some TSK_R) (Cons None (Cons (Some TSK_R) (append (replicate 2 None) []))))))))) [] TyTrLeaf [Some abbreviatedType1] (TyTrSplit (Cons (Some TSK_R) (Cons None (Cons (Some TSK_R) (Cons (Some TSK_R) (Cons (Some TSK_R) (Cons None (Cons (Some TSK_L) (Cons None (Cons (Some TSK_L) (append (replicate 2 None) [])))))))))) [] TyTrLeaf [Some abbreviatedType2] (TyTrSplit (Cons (Some TSK_L) (Cons (Some TSK_L) (Cons None (Cons (Some TSK_L) (Cons (Some TSK_L) (Cons (Some TSK_L) (append (replicate 6 None) []))))))) [] TyTrLeaf [Some (TRecord [(''n'', (TPrim (Num U64), Present)), (''stop'', (TFun abbreviatedType3 (TPrim Bool), Present)), (''step'', (TFun abbreviatedType3 abbreviatedType1, Present)), (''acc'', (abbreviatedType1, Present)), (''obsv'', (abbreviatedType2, Present))] Unboxed)] (TyTrSplit (Cons (Some TSK_L) (append (replicate 12 None) [])) [] TyTrLeaf [Some abbreviatedType1] (TyTrSplit (Cons (Some TSK_L) (append (replicate 13 None) [])) [] TyTrLeaf [Some (TPrim (Num U32)), Some (TRecord [(''p1'', (TPrim (Num U32), Taken)), (''p2'', (TPrim (Num U32), Present))] Unboxed)] (TyTrSplit (Cons (Some TSK_R) (Cons (Some TSK_L) (append (replicate 14 None) []))) [] TyTrLeaf [Some (TPrim (Num U32)), Some (TRecord [(''p1'', (TPrim (Num U32), Taken)), (''p2'', (TPrim (Num U32), Taken))] Unboxed)] TyTrLeaf))))))))))))"
+  "binarySearch_typetree \<equiv> TyTrSplit (Cons (Some TSK_L) []) [] TyTrLeaf [Some (TCon ''WordArray'' [TPrim (Num U32)] (Boxed ReadOnly undefined)), Some (TRecord [(''p1'', (TCon ''WordArray'' [TPrim (Num U32)] (Boxed ReadOnly undefined), Taken)), (''p2'', (TPrim (Num U32), Present))] Unboxed)] (TyTrSplit (Cons (Some TSK_R) (Cons (Some TSK_L) (Cons None []))) [] TyTrLeaf [Some (TPrim (Num U32)), Some (TRecord [(''p1'', (TCon ''WordArray'' [TPrim (Num U32)] (Boxed ReadOnly undefined), Taken)), (''p2'', (TPrim (Num U32), Taken))] Unboxed)] (TyTrSplit (Cons (Some TSK_R) (Cons (Some TSK_L) (Cons (Some TSK_S) (append (replicate 2 None) [])))) [] TyTrLeaf [Some (TPrim (Num U32))] (TyTrSplit (Cons (Some TSK_S) (Cons (Some TSK_R) (Cons None (Cons (Some TSK_R) (append (replicate 2 None) []))))) [] TyTrLeaf [Some (TPrim (Num U64))] (TyTrSplit (Cons (Some TSK_R) (Cons (Some TSK_R) (Cons (Some TSK_R) (Cons None (Cons (Some TSK_R) (append (replicate 2 None) [])))))) [] TyTrLeaf [Some (TFun abbreviatedType4 (TPrim Bool))] (TyTrSplit (Cons (Some TSK_R) (Cons (Some TSK_R) (Cons (Some TSK_R) (Cons (Some TSK_R) (Cons None (Cons (Some TSK_R) (append (replicate 2 None) []))))))) [] TyTrLeaf [Some (TFun abbreviatedType4 abbreviatedType3)] (TyTrSplit (Cons (Some TSK_R) (Cons (Some TSK_R) (Cons (Some TSK_R) (Cons (Some TSK_R) (Cons (Some TSK_R) (Cons None (Cons (Some TSK_R) (append (replicate 2 None) [])))))))) [] TyTrLeaf [Some (TPrim (Num U32))] (TyTrSplit (Cons (Some TSK_R) (Cons (Some TSK_R) (Cons (Some TSK_R) (Cons (Some TSK_R) (Cons (Some TSK_R) (Cons (Some TSK_R) (Cons None (Cons (Some TSK_R) (append (replicate 2 None) []))))))))) [] TyTrLeaf [Some (TPrim Bool)] (TyTrSplit (Cons (Some TSK_L) (Cons (Some TSK_L) (Cons (Some TSK_R) (Cons (Some TSK_R) (Cons (Some TSK_R) (Cons (Some TSK_S) (Cons (Some TSK_R) (Cons None (Cons (Some TSK_R) (append (replicate 2 None) [])))))))))) [] TyTrLeaf [Some abbreviatedType3] (TyTrSplit (Cons (Some TSK_R) (append (replicate 2 None) (Cons (Some TSK_R) (Cons (Some TSK_R) (Cons (Some TSK_R) (Cons (Some TSK_R) (Cons (Some TSK_L) (Cons None (Cons (Some TSK_L) (append (replicate 2 None) [])))))))))) [] TyTrLeaf [Some abbreviatedType2] (TyTrSplit (Cons (Some TSK_L) (Cons (Some TSK_L) (append (replicate 2 None) (Cons (Some TSK_L) (Cons (Some TSK_L) (Cons (Some TSK_L) (Cons (Some TSK_R) (append (replicate 5 None) [])))))))) [] TyTrLeaf [Some (TRecord [(''n'', (TPrim (Num U64), Present)), (''stop'', (TFun abbreviatedType4 (TPrim Bool), Present)), (''step'', (TFun abbreviatedType4 abbreviatedType3, Present)), (''acc'', (abbreviatedType3, Present)), (''obsv'', (abbreviatedType2, Present))] Unboxed)] (TyTrSplit (Cons (Some TSK_L) (append (replicate 7 None) (Cons (Some TSK_R) (append (replicate 5 None) [])))) [] TyTrLeaf [Some abbreviatedType3] (TyTrSplit (Cons (Some TSK_L) (append (replicate 8 None) (Cons (Some TSK_R) (append (replicate 5 None) [])))) [] TyTrLeaf [Some (TPrim (Num U32)), Some (TRecord [(''p1'', (TPrim (Num U32), Taken)), (''p2'', (TPrim (Num U32), Present)), (''p3'', (TPrim Bool, Present))] Unboxed)] (TyTrSplit (Cons (Some TSK_R) (Cons (Some TSK_L) (append (replicate 9 None) (Cons (Some TSK_R) (append (replicate 5 None) []))))) [] TyTrLeaf [Some (TPrim (Num U32)), Some (TRecord [(''p1'', (TPrim (Num U32), Taken)), (''p2'', (TPrim (Num U32), Taken)), (''p3'', (TPrim Bool, Present))] Unboxed)] (TyTrSplit (Cons (Some TSK_L) (Cons (Some TSK_L) (Cons (Some TSK_R) (append (replicate 10 None) (Cons (Some TSK_R) (append (replicate 5 None) [])))))) [] TyTrLeaf [Some (TPrim Bool), Some (TRecord [(''p1'', (TPrim (Num U32), Taken)), (''p2'', (TPrim (Num U32), Taken)), (''p3'', (TPrim Bool, Taken))] Unboxed)] (TyTrSplit (Cons (Some TSK_L) (Cons (Some TSK_L) (append (replicate 2 None) (Cons (Some TSK_R) (append (replicate 10 None) (Cons (Some TSK_R) (append (replicate 5 None) []))))))) [] TyTrLeaf [] (TyTrSplit (append (replicate 4 None) (Cons (Some TSK_S) (append (replicate 10 None) (Cons (Some TSK_S) (append (replicate 5 None) []))))) [] TyTrLeaf [] TyTrLeaf))))))))))))))))"
 
 definition
-  "myexp_typetree \<equiv> TyTrSplit (Cons (Some TSK_L) []) [] TyTrLeaf [Some (TPrim (Num U32)), Some (TRecord [(''p1'', (TPrim (Num U32), Taken)), (''p2'', (TPrim (Num U32), Present))] Unboxed)] (TyTrSplit (Cons (Some TSK_R) (Cons (Some TSK_L) (Cons None []))) [] TyTrLeaf [Some (TPrim (Num U32)), Some (TRecord [(''p1'', (TPrim (Num U32), Taken)), (''p2'', (TPrim (Num U32), Taken))] Unboxed)] (TyTrSplit (Cons (Some TSK_L) (Cons (Some TSK_L) (Cons (Some TSK_R) (append (replicate 2 None) [])))) [] TyTrLeaf [Some (TPrim (Num U64))] (TyTrSplit (Cons (Some TSK_R) (append (replicate 2 None) (Cons (Some TSK_R) (append (replicate 2 None) [])))) [] TyTrLeaf [Some (TFun abbreviatedType6 (TPrim Bool))] (TyTrSplit (Cons (Some TSK_R) (Cons (Some TSK_R) (append (replicate 2 None) (Cons (Some TSK_R) (append (replicate 2 None) []))))) [] TyTrLeaf [Some (TFun abbreviatedType6 (TPrim (Num U32)))] (TyTrSplit (Cons (Some TSK_R) (Cons (Some TSK_R) (Cons (Some TSK_R) (append (replicate 2 None) (Cons (Some TSK_R) (append (replicate 2 None) [])))))) [] TyTrLeaf [Some (TPrim (Num U32))] (TyTrSplit (Cons (Some TSK_L) (Cons (Some TSK_L) (Cons (Some TSK_L) (Cons (Some TSK_L) (append (replicate 2 None) (Cons (Some TSK_L) (append (replicate 2 None) []))))))) [] TyTrLeaf [Some (TRecord [(''n'', (TPrim (Num U64), Present)), (''stop'', (TFun abbreviatedType6 (TPrim Bool), Present)), (''step'', (TFun abbreviatedType6 (TPrim (Num U32)), Present)), (''acc'', (TPrim (Num U32), Present)), (''obsv'', (TPrim (Num U32), Present))] Unboxed)] TyTrLeaf))))))"
+  "myexp_typetree \<equiv> TyTrSplit (Cons (Some TSK_L) []) [] TyTrLeaf [Some (TPrim (Num U32)), Some (TRecord [(''p1'', (TPrim (Num U32), Taken)), (''p2'', (TPrim (Num U32), Present))] Unboxed)] (TyTrSplit (Cons (Some TSK_R) (Cons (Some TSK_L) (Cons None []))) [] TyTrLeaf [Some (TPrim (Num U32)), Some (TRecord [(''p1'', (TPrim (Num U32), Taken)), (''p2'', (TPrim (Num U32), Taken))] Unboxed)] (TyTrSplit (Cons (Some TSK_L) (Cons (Some TSK_L) (Cons (Some TSK_R) (append (replicate 2 None) [])))) [] TyTrLeaf [Some (TPrim (Num U64))] (TyTrSplit (Cons (Some TSK_R) (append (replicate 2 None) (Cons (Some TSK_R) (append (replicate 2 None) [])))) [] TyTrLeaf [Some (TFun abbreviatedType7 (TPrim Bool))] (TyTrSplit (Cons (Some TSK_R) (Cons (Some TSK_R) (append (replicate 2 None) (Cons (Some TSK_R) (append (replicate 2 None) []))))) [] TyTrLeaf [Some (TFun abbreviatedType7 (TPrim (Num U32)))] (TyTrSplit (Cons (Some TSK_R) (Cons (Some TSK_R) (Cons (Some TSK_R) (append (replicate 2 None) (Cons (Some TSK_R) (append (replicate 2 None) [])))))) [] TyTrLeaf [Some (TPrim (Num U32))] (TyTrSplit (Cons (Some TSK_L) (Cons (Some TSK_L) (Cons (Some TSK_L) (Cons (Some TSK_L) (append (replicate 2 None) (Cons (Some TSK_L) (append (replicate 2 None) []))))))) [] TyTrLeaf [Some (TRecord [(''n'', (TPrim (Num U64), Present)), (''stop'', (TFun abbreviatedType7 (TPrim Bool), Present)), (''step'', (TFun abbreviatedType7 (TPrim (Num U32)), Present)), (''acc'', (TPrim (Num U32), Present)), (''obsv'', (TPrim (Num U32), Present))] Unboxed)] TyTrLeaf))))))"
 
 definition
-  "mylog2_typetree \<equiv> TyTrSplit (Cons (Some TSK_L) []) [] TyTrLeaf [Some (TPrim (Num U64))] (TyTrSplit (Cons (Some TSK_R) (Cons None [])) [] TyTrLeaf [Some (TFun abbreviatedType5 (TPrim Bool))] (TyTrSplit (Cons (Some TSK_R) (Cons (Some TSK_R) (Cons None []))) [] TyTrLeaf [Some (TFun abbreviatedType5 abbreviatedType4)] (TyTrSplit (Cons (Some TSK_R) (Cons (Some TSK_R) (Cons (Some TSK_R) (Cons None [])))) [] TyTrLeaf [Some (TPrim (Num U64))] (TyTrSplit (Cons (Some TSK_R) (Cons (Some TSK_R) (Cons (Some TSK_R) (Cons (Some TSK_R) (Cons None []))))) [] TyTrLeaf [Some (TPrim (Num U64))] (TyTrSplit (Cons (Some TSK_L) (Cons (Some TSK_L) (Cons (Some TSK_R) (Cons (Some TSK_R) (Cons (Some TSK_R) (Cons None [])))))) [] TyTrLeaf [Some abbreviatedType4] (TyTrSplit (Cons (Some TSK_L) (append (replicate 2 None) (Cons (Some TSK_L) (Cons (Some TSK_L) (Cons (Some TSK_L) (Cons None [])))))) [] TyTrLeaf [Some (TRecord [(''n'', (TPrim (Num U64), Present)), (''stop'', (TFun abbreviatedType5 (TPrim Bool), Present)), (''step'', (TFun abbreviatedType5 abbreviatedType4, Present)), (''acc'', (abbreviatedType4, Present)), (''obsv'', (TPrim (Num U64), Present))] Unboxed)] (TyTrSplit (Cons (Some TSK_L) (append (replicate 7 None) [])) [] TyTrLeaf [Some abbreviatedType4] (TyTrSplit (Cons (Some TSK_L) (append (replicate 8 None) [])) [] TyTrLeaf [Some (TPrim (Num U64)), Some (TRecord [(''p1'', (TPrim (Num U64), Taken)), (''p2'', (TPrim (Num U64), Present))] Unboxed)] (TyTrSplit (Cons (Some TSK_L) (Cons (Some TSK_L) (append (replicate 9 None) []))) [] TyTrLeaf [Some (TPrim (Num U64)), Some (TRecord [(''p1'', (TPrim (Num U64), Taken)), (''p2'', (TPrim (Num U64), Taken))] Unboxed)] TyTrLeaf)))))))))"
+  "mylog2_typetree \<equiv> TyTrSplit (Cons (Some TSK_L) []) [] TyTrLeaf [Some (TPrim (Num U64))] (TyTrSplit (Cons (Some TSK_R) (Cons None [])) [] TyTrLeaf [Some (TFun abbreviatedType6 (TPrim Bool))] (TyTrSplit (Cons (Some TSK_R) (Cons (Some TSK_R) (Cons None []))) [] TyTrLeaf [Some (TFun abbreviatedType6 abbreviatedType5)] (TyTrSplit (Cons (Some TSK_R) (Cons (Some TSK_R) (Cons (Some TSK_R) (Cons None [])))) [] TyTrLeaf [Some (TPrim (Num U64))] (TyTrSplit (Cons (Some TSK_R) (Cons (Some TSK_R) (Cons (Some TSK_R) (Cons (Some TSK_R) (Cons None []))))) [] TyTrLeaf [Some (TPrim (Num U64))] (TyTrSplit (Cons (Some TSK_L) (Cons (Some TSK_L) (Cons (Some TSK_R) (Cons (Some TSK_R) (Cons (Some TSK_R) (Cons None [])))))) [] TyTrLeaf [Some abbreviatedType5] (TyTrSplit (Cons (Some TSK_L) (append (replicate 2 None) (Cons (Some TSK_L) (Cons (Some TSK_L) (Cons (Some TSK_L) (Cons None [])))))) [] TyTrLeaf [Some (TRecord [(''n'', (TPrim (Num U64), Present)), (''stop'', (TFun abbreviatedType6 (TPrim Bool), Present)), (''step'', (TFun abbreviatedType6 abbreviatedType5, Present)), (''acc'', (abbreviatedType5, Present)), (''obsv'', (TPrim (Num U64), Present))] Unboxed)] (TyTrSplit (Cons (Some TSK_L) (append (replicate 7 None) [])) [] TyTrLeaf [Some abbreviatedType5] (TyTrSplit (Cons (Some TSK_L) (append (replicate 8 None) [])) [] TyTrLeaf [Some (TPrim (Num U64)), Some (TRecord [(''p1'', (TPrim (Num U64), Taken)), (''p2'', (TPrim (Num U64), Present))] Unboxed)] (TyTrSplit (Cons (Some TSK_L) (Cons (Some TSK_L) (append (replicate 9 None) []))) [] TyTrLeaf [Some (TPrim (Num U64)), Some (TRecord [(''p1'', (TPrim (Num U64), Taken)), (''p2'', (TPrim (Num U64), Taken))] Unboxed)] TyTrLeaf)))))))))"
 
 ML \<open> open TTyping_Tactics \<close>
 
@@ -210,7 +216,7 @@ val typing_helper_1_script : tac list = [
 
 
 lemma typing_helper_1[unfolded abbreviated_type_defs] :
-  "kinding [] abbreviatedType6 {E, S, D}"
+  "kinding [] abbreviatedType7 {E, S, D}"
   apply (unfold abbreviated_type_defs)?
   apply (tactic \<open> map (fn t => DETERM (interpret_tac t @{context} 1)) typing_helper_1_script |> EVERY \<close>)
   done
@@ -222,7 +228,7 @@ val typing_helper_2_script : tac list = [
 
 
 lemma typing_helper_2[unfolded abbreviated_type_defs] :
-  "kinding [] abbreviatedType5 {E, S, D}"
+  "kinding [] abbreviatedType6 {E, S, D}"
   apply (unfold abbreviated_type_defs)?
   apply (tactic \<open> map (fn t => DETERM (interpret_tac t @{context} 1)) typing_helper_2_script |> EVERY \<close>)
   done
@@ -234,7 +240,7 @@ val typing_helper_3_script : tac list = [
 
 
 lemma typing_helper_3[unfolded abbreviated_type_defs] :
-  "kinding [] abbreviatedType4 {E, S, D}"
+  "kinding [] abbreviatedType5 {E, S, D}"
   apply (unfold abbreviated_type_defs)?
   apply (tactic \<open> map (fn t => DETERM (interpret_tac t @{context} 1)) typing_helper_3_script |> EVERY \<close>)
   done
@@ -246,7 +252,7 @@ val typing_helper_4_script : tac list = [
 
 
 lemma typing_helper_4[unfolded abbreviated_type_defs] :
-  "kinding [] (TRecord [(''acc'', (abbreviatedType4, Taken)), (''obsv'', (TPrim (Num U64), Present))] Unboxed) {E, S, D}"
+  "kinding [] (TRecord [(''acc'', (abbreviatedType5, Taken)), (''obsv'', (TPrim (Num U64), Present))] Unboxed) {E, S, D}"
   apply (unfold abbreviated_type_defs)?
   apply (tactic \<open> map (fn t => DETERM (interpret_tac t @{context} 1)) typing_helper_4_script |> EVERY \<close>)
   done
@@ -270,7 +276,7 @@ val typing_helper_6_script : tac list = [
 
 
 lemma typing_helper_6[unfolded abbreviated_type_defs] :
-  "kinding [] (TRecord [(''acc'', (abbreviatedType4, Taken)), (''obsv'', (TPrim (Num U64), Taken))] Unboxed) {E, S, D}"
+  "kinding [] (TRecord [(''acc'', (abbreviatedType5, Taken)), (''obsv'', (TPrim (Num U64), Taken))] Unboxed) {E, S, D}"
   apply (unfold abbreviated_type_defs)?
   apply (tactic \<open> map (fn t => DETERM (interpret_tac t @{context} 1)) typing_helper_6_script |> EVERY \<close>)
   done
@@ -306,7 +312,7 @@ val typing_helper_9_script : tac list = [
 
 
 lemma typing_helper_9[unfolded abbreviated_type_defs] :
-  "kinding [] abbreviatedType3 {S, D}"
+  "kinding [] abbreviatedType4 {S, D}"
   apply (unfold abbreviated_type_defs)?
   apply (tactic \<open> map (fn t => DETERM (interpret_tac t @{context} 1)) typing_helper_9_script |> EVERY \<close>)
   done
@@ -318,7 +324,7 @@ val typing_helper_10_script : tac list = [
 
 
 lemma typing_helper_10[unfolded abbreviated_type_defs] :
-  "kinding [] abbreviatedType1 {E, S, D}"
+  "kinding [] abbreviatedType3 {E, S, D}"
   apply (unfold abbreviated_type_defs)?
   apply (tactic \<open> map (fn t => DETERM (interpret_tac t @{context} 1)) typing_helper_10_script |> EVERY \<close>)
   done
@@ -330,7 +336,7 @@ val typing_helper_11_script : tac list = [
 
 
 lemma typing_helper_11[unfolded abbreviated_type_defs] :
-  "kinding [] (TRecord [(''acc'', (abbreviatedType1, Taken)), (''obsv'', (abbreviatedType2, Present))] Unboxed) {S, D}"
+  "kinding [] (TRecord [(''acc'', (abbreviatedType3, Taken)), (''obsv'', (abbreviatedType2, Present))] Unboxed) {S, D}"
   apply (unfold abbreviated_type_defs)?
   apply (tactic \<open> map (fn t => DETERM (interpret_tac t @{context} 1)) typing_helper_11_script |> EVERY \<close>)
   done
@@ -354,7 +360,7 @@ val typing_helper_13_script : tac list = [
 
 
 lemma typing_helper_13[unfolded abbreviated_type_defs] :
-  "kinding [] (TRecord [(''acc'', (abbreviatedType1, Taken)), (''obsv'', (abbreviatedType2, Taken))] Unboxed) {E, S, D}"
+  "kinding [] (TRecord [(''acc'', (abbreviatedType3, Taken)), (''obsv'', (abbreviatedType2, Taken))] Unboxed) {E, S, D}"
   apply (unfold abbreviated_type_defs)?
   apply (tactic \<open> map (fn t => DETERM (interpret_tac t @{context} 1)) typing_helper_13_script |> EVERY \<close>)
   done
@@ -378,7 +384,7 @@ val typing_helper_15_script : tac list = [
 
 
 lemma typing_helper_15[unfolded abbreviated_type_defs] :
-  "kinding [] (TRecord [(''p1'', (TPrim (Num U32), Taken)), (''p2'', (TPrim (Num U32), Present))] Unboxed) {E, S, D}"
+  "kinding [] (TRecord [(''p1'', (TPrim (Num U32), Taken)), (''p2'', (TPrim (Num U32), Present)), (''p3'', (TPrim Bool, Present))] Unboxed) {E, S, D}"
   apply (unfold abbreviated_type_defs)?
   apply (tactic \<open> map (fn t => DETERM (interpret_tac t @{context} 1)) typing_helper_15_script |> EVERY \<close>)
   done
@@ -390,7 +396,7 @@ val typing_helper_16_script : tac list = [
 
 
 lemma typing_helper_16[unfolded abbreviated_type_defs] :
-  "kinding [] (TRecord [(''p1'', (TPrim (Num U32), Taken)), (''p2'', (TPrim (Num U32), Taken))] Unboxed) {E, S, D}"
+  "kinding [] (TRecord [(''p1'', (TPrim (Num U32), Taken)), (''p2'', (TPrim (Num U32), Taken)), (''p3'', (TPrim Bool, Present))] Unboxed) {E, S, D}"
   apply (unfold abbreviated_type_defs)?
   apply (tactic \<open> map (fn t => DETERM (interpret_tac t @{context} 1)) typing_helper_16_script |> EVERY \<close>)
   done
@@ -402,7 +408,7 @@ val typing_helper_17_script : tac list = [
 
 
 lemma typing_helper_17[unfolded abbreviated_type_defs] :
-  "kinding [] (TCon ''WordArray'' [TPrim (Num U32)] (Boxed ReadOnly undefined)) {S, D}"
+  "kinding [] (TPrim Bool) {E, S, D}"
   apply (unfold abbreviated_type_defs)?
   apply (tactic \<open> map (fn t => DETERM (interpret_tac t @{context} 1)) typing_helper_17_script |> EVERY \<close>)
   done
@@ -414,7 +420,7 @@ val typing_helper_18_script : tac list = [
 
 
 lemma typing_helper_18[unfolded abbreviated_type_defs] :
-  "kinding [] (TRecord [(''p1'', (TCon ''WordArray'' [TPrim (Num U32)] (Boxed ReadOnly undefined), Taken)), (''p2'', (TPrim (Num U32), Present))] Unboxed) {E, S, D}"
+  "kinding [] (TRecord [(''p1'', (TPrim (Num U32), Taken)), (''p2'', (TPrim (Num U32), Taken)), (''p3'', (TPrim Bool, Taken))] Unboxed) {E, S, D}"
   apply (unfold abbreviated_type_defs)?
   apply (tactic \<open> map (fn t => DETERM (interpret_tac t @{context} 1)) typing_helper_18_script |> EVERY \<close>)
   done
@@ -426,91 +432,91 @@ val typing_helper_19_script : tac list = [
 
 
 lemma typing_helper_19[unfolded abbreviated_type_defs] :
-  "kinding [] (TRecord [(''p1'', (TCon ''WordArray'' [TPrim (Num U32)] (Boxed ReadOnly undefined), Taken)), (''p2'', (TPrim (Num U32), Taken))] Unboxed) {E, S, D}"
+  "kinding [] (TRecord [(''acc'', (TPrim (Num U32), Taken)), (''obsv'', (TPrim (Num U32), Present))] Unboxed) {E, S, D}"
   apply (unfold abbreviated_type_defs)?
   apply (tactic \<open> map (fn t => DETERM (interpret_tac t @{context} 1)) typing_helper_19_script |> EVERY \<close>)
   done
 
 ML_quiet \<open>
 val typing_helper_20_script : tac list = [
-(ForceTac [])
+(ForceTac [@{thm kinding_def},@{thm kinding_all_def},@{thm kinding_variant_def},@{thm kinding_record_def}])
 ] \<close>
 
 
 lemma typing_helper_20[unfolded abbreviated_type_defs] :
-  "type_wellformed 0 (TPrim (Num U32))"
+  "kinding [] (TRecord [(''acc'', (TPrim (Num U32), Taken)), (''obsv'', (TPrim (Num U32), Taken))] Unboxed) {E, S, D}"
   apply (unfold abbreviated_type_defs)?
   apply (tactic \<open> map (fn t => DETERM (interpret_tac t @{context} 1)) typing_helper_20_script |> EVERY \<close>)
   done
 
 ML_quiet \<open>
 val typing_helper_21_script : tac list = [
-(ForceTac [])
+(ForceTac [@{thm kinding_def},@{thm kinding_all_def},@{thm kinding_variant_def},@{thm kinding_record_def}])
 ] \<close>
 
 
 lemma typing_helper_21[unfolded abbreviated_type_defs] :
-  "type_wellformed 0 (TRecord [(''p1'', (TCon ''WordArray'' [TPrim (Num U32)] (Boxed ReadOnly undefined), Taken)), (''p2'', (TPrim (Num U32), Taken))] Unboxed)"
+  "kinding [] (TCon ''WordArray'' [TPrim (Num U32)] (Boxed ReadOnly undefined)) {S, D}"
   apply (unfold abbreviated_type_defs)?
   apply (tactic \<open> map (fn t => DETERM (interpret_tac t @{context} 1)) typing_helper_21_script |> EVERY \<close>)
   done
 
 ML_quiet \<open>
 val typing_helper_22_script : tac list = [
-(ForceTac [])
+(ForceTac [@{thm kinding_def},@{thm kinding_all_def},@{thm kinding_variant_def},@{thm kinding_record_def}])
 ] \<close>
 
 
 lemma typing_helper_22[unfolded abbreviated_type_defs] :
-  "type_wellformed 0 (TCon ''WordArray'' [TPrim (Num U32)] (Boxed ReadOnly undefined))"
+  "kinding [] (TRecord [(''p1'', (TCon ''WordArray'' [TPrim (Num U32)] (Boxed ReadOnly undefined), Taken)), (''p2'', (TPrim (Num U32), Present))] Unboxed) {E, S, D}"
   apply (unfold abbreviated_type_defs)?
   apply (tactic \<open> map (fn t => DETERM (interpret_tac t @{context} 1)) typing_helper_22_script |> EVERY \<close>)
   done
 
 ML_quiet \<open>
 val typing_helper_23_script : tac list = [
-(SimpTac ([],[(nth @{thms HOL.simp_thms} (25-1)),(nth @{thms HOL.simp_thms} (26-1))]))
+(ForceTac [@{thm kinding_def},@{thm kinding_all_def},@{thm kinding_variant_def},@{thm kinding_record_def}])
 ] \<close>
 
 
 lemma typing_helper_23[unfolded abbreviated_type_defs] :
-  "list_all2 (kinding []) [] []"
+  "kinding [] (TRecord [(''p1'', (TCon ''WordArray'' [TPrim (Num U32)] (Boxed ReadOnly undefined), Taken)), (''p2'', (TPrim (Num U32), Taken))] Unboxed) {E, S, D}"
   apply (unfold abbreviated_type_defs)?
   apply (tactic \<open> map (fn t => DETERM (interpret_tac t @{context} 1)) typing_helper_23_script |> EVERY \<close>)
   done
 
 ML_quiet \<open>
 val typing_helper_24_script : tac list = [
-(ForceTac [])
+(ForceTac [@{thm kinding_def},@{thm kinding_all_def},@{thm kinding_variant_def},@{thm kinding_record_def}])
 ] \<close>
 
 
 lemma typing_helper_24[unfolded abbreviated_type_defs] :
-  "type_wellformed 0 (TFun (TCon ''WordArray'' [TPrim (Num U32)] (Boxed ReadOnly undefined)) (TPrim (Num U32)))"
+  "kinding [] (TRecord [(''arr'', (TCon ''WordArray'' [TPrim (Num U32)] (Boxed ReadOnly undefined), Present)), (''idx'', (TPrim (Num U32), Present)), (''val'', (TPrim (Num U32), Present))] Unboxed) {S, D}"
   apply (unfold abbreviated_type_defs)?
   apply (tactic \<open> map (fn t => DETERM (interpret_tac t @{context} 1)) typing_helper_24_script |> EVERY \<close>)
   done
 
 ML_quiet \<open>
 val typing_helper_25_script : tac list = [
-(ForceTac [@{thm kinding_def},@{thm kinding_all_def},@{thm kinding_variant_def},@{thm kinding_record_def}])
+(ForceTac [])
 ] \<close>
 
 
 lemma typing_helper_25[unfolded abbreviated_type_defs] :
-  "kinding [] (TRecord [(''arr'', (TCon ''WordArray'' [TPrim (Num U32)] (Boxed ReadOnly undefined), Present)), (''idx'', (TPrim (Num U32), Present)), (''val'', (TPrim (Num U32), Present))] Unboxed) {S, D}"
+  "type_wellformed 0 (TRecord [(''arr'', (TCon ''WordArray'' [TPrim (Num U32)] (Boxed ReadOnly undefined), Present)), (''idx'', (TPrim (Num U32), Present)), (''val'', (TPrim (Num U32), Present))] Unboxed)"
   apply (unfold abbreviated_type_defs)?
   apply (tactic \<open> map (fn t => DETERM (interpret_tac t @{context} 1)) typing_helper_25_script |> EVERY \<close>)
   done
 
 ML_quiet \<open>
 val typing_helper_26_script : tac list = [
-(ForceTac [])
+(SimpTac ([],[(nth @{thms HOL.simp_thms} (25-1)),(nth @{thms HOL.simp_thms} (26-1))]))
 ] \<close>
 
 
 lemma typing_helper_26[unfolded abbreviated_type_defs] :
-  "type_wellformed 0 (TRecord [(''arr'', (TCon ''WordArray'' [TPrim (Num U32)] (Boxed ReadOnly undefined), Present)), (''idx'', (TPrim (Num U32), Present)), (''val'', (TPrim (Num U32), Present))] Unboxed)"
+  "list_all2 (kinding []) [] []"
   apply (unfold abbreviated_type_defs)?
   apply (tactic \<open> map (fn t => DETERM (interpret_tac t @{context} 1)) typing_helper_26_script |> EVERY \<close>)
   done
@@ -529,36 +535,36 @@ lemma typing_helper_27[unfolded abbreviated_type_defs] :
 
 ML_quiet \<open>
 val typing_helper_28_script : tac list = [
-(ForceTac [@{thm kinding_def},@{thm kinding_all_def},@{thm kinding_variant_def},@{thm kinding_record_def}])
+(ForceTac [])
 ] \<close>
 
 
 lemma typing_helper_28[unfolded abbreviated_type_defs] :
-  "kinding [] (TPrim Bool) {E, S, D}"
+  "type_wellformed 0 (TRecord [(''p1'', (TCon ''WordArray'' [TPrim (Num U32)] (Boxed ReadOnly undefined), Taken)), (''p2'', (TPrim (Num U32), Taken))] Unboxed)"
   apply (unfold abbreviated_type_defs)?
   apply (tactic \<open> map (fn t => DETERM (interpret_tac t @{context} 1)) typing_helper_28_script |> EVERY \<close>)
   done
 
 ML_quiet \<open>
 val typing_helper_29_script : tac list = [
-(ForceTac [@{thm kinding_def},@{thm kinding_all_def},@{thm kinding_variant_def},@{thm kinding_record_def}])
+(ForceTac [])
 ] \<close>
 
 
 lemma typing_helper_29[unfolded abbreviated_type_defs] :
-  "kinding [] (TRecord [(''acc'', (TPrim (Num U32), Taken)), (''obsv'', (TPrim (Num U32), Present))] Unboxed) {E, S, D}"
+  "type_wellformed 0 (TCon ''WordArray'' [TPrim (Num U32)] (Boxed ReadOnly undefined))"
   apply (unfold abbreviated_type_defs)?
   apply (tactic \<open> map (fn t => DETERM (interpret_tac t @{context} 1)) typing_helper_29_script |> EVERY \<close>)
   done
 
 ML_quiet \<open>
 val typing_helper_30_script : tac list = [
-(ForceTac [@{thm kinding_def},@{thm kinding_all_def},@{thm kinding_variant_def},@{thm kinding_record_def}])
+(ForceTac [])
 ] \<close>
 
 
 lemma typing_helper_30[unfolded abbreviated_type_defs] :
-  "kinding [] (TRecord [(''acc'', (TPrim (Num U32), Taken)), (''obsv'', (TPrim (Num U32), Taken))] Unboxed) {E, S, D}"
+  "type_wellformed 0 (TFun (TCon ''WordArray'' [TPrim (Num U32)] (Boxed ReadOnly undefined)) (TPrim (Num U32)))"
   apply (unfold abbreviated_type_defs)?
   apply (tactic \<open> map (fn t => DETERM (interpret_tac t @{context} 1)) typing_helper_30_script |> EVERY \<close>)
   done
@@ -570,7 +576,7 @@ val typing_helper_31_script : tac list = [
 
 
 lemma typing_helper_31[unfolded abbreviated_type_defs] :
-  "kinding [] (TFun abbreviatedType3 (TPrim Bool)) {E, S, D}"
+  "kinding [] (TFun abbreviatedType4 (TPrim Bool)) {E, S, D}"
   apply (unfold abbreviated_type_defs)?
   apply (tactic \<open> map (fn t => DETERM (interpret_tac t @{context} 1)) typing_helper_31_script |> EVERY \<close>)
   done
@@ -582,7 +588,7 @@ val typing_helper_32_script : tac list = [
 
 
 lemma typing_helper_32[unfolded abbreviated_type_defs] :
-  "type_wellformed 0 abbreviatedType3"
+  "type_wellformed 0 abbreviatedType4"
   apply (unfold abbreviated_type_defs)?
   apply (tactic \<open> map (fn t => DETERM (interpret_tac t @{context} 1)) typing_helper_32_script |> EVERY \<close>)
   done
@@ -594,7 +600,7 @@ val typing_helper_33_script : tac list = [
 
 
 lemma typing_helper_33[unfolded abbreviated_type_defs] :
-  "kinding [] (TFun abbreviatedType3 abbreviatedType1) {E, S, D}"
+  "kinding [] (TFun abbreviatedType4 abbreviatedType3) {E, S, D}"
   apply (unfold abbreviated_type_defs)?
   apply (tactic \<open> map (fn t => DETERM (interpret_tac t @{context} 1)) typing_helper_33_script |> EVERY \<close>)
   done
@@ -606,7 +612,7 @@ val typing_helper_34_script : tac list = [
 
 
 lemma typing_helper_34[unfolded abbreviated_type_defs] :
-  "kinding [] (TRecord [(''n'', (TPrim (Num U64), Present)), (''stop'', (TFun abbreviatedType3 (TPrim Bool), Present)), (''step'', (TFun abbreviatedType3 abbreviatedType1, Present)), (''acc'', (abbreviatedType1, Present)), (''obsv'', (abbreviatedType2, Present))] Unboxed) {S, D}"
+  "kinding [] (TRecord [(''n'', (TPrim (Num U64), Present)), (''stop'', (TFun abbreviatedType4 (TPrim Bool), Present)), (''step'', (TFun abbreviatedType4 abbreviatedType3, Present)), (''acc'', (abbreviatedType3, Present)), (''obsv'', (abbreviatedType2, Present))] Unboxed) {S, D}"
   apply (unfold abbreviated_type_defs)?
   apply (tactic \<open> map (fn t => DETERM (interpret_tac t @{context} 1)) typing_helper_34_script |> EVERY \<close>)
   done
@@ -618,7 +624,7 @@ val typing_helper_35_script : tac list = [
 
 
 lemma typing_helper_35[unfolded abbreviated_type_defs] :
-  "type_wellformed 0 (TRecord [(''n'', (TPrim (Num U64), Present)), (''stop'', (TFun abbreviatedType3 (TPrim Bool), Present)), (''step'', (TFun abbreviatedType3 abbreviatedType1, Present)), (''acc'', (abbreviatedType1, Present)), (''obsv'', (abbreviatedType2, Present))] Unboxed)"
+  "type_wellformed 0 (TRecord [(''n'', (TPrim (Num U64), Present)), (''stop'', (TFun abbreviatedType4 (TPrim Bool), Present)), (''step'', (TFun abbreviatedType4 abbreviatedType3, Present)), (''acc'', (abbreviatedType3, Present)), (''obsv'', (abbreviatedType2, Present))] Unboxed)"
   apply (unfold abbreviated_type_defs)?
   apply (tactic \<open> map (fn t => DETERM (interpret_tac t @{context} 1)) typing_helper_35_script |> EVERY \<close>)
   done
@@ -630,7 +636,7 @@ val typing_helper_36_script : tac list = [
 
 
 lemma typing_helper_36[unfolded abbreviated_type_defs] :
-  "type_wellformed 0 (TFun (TRecord [(''n'', (TPrim (Num U64), Present)), (''stop'', (TFun abbreviatedType3 (TPrim Bool), Present)), (''step'', (TFun abbreviatedType3 abbreviatedType1, Present)), (''acc'', (abbreviatedType1, Present)), (''obsv'', (abbreviatedType2, Present))] Unboxed) abbreviatedType1)"
+  "type_wellformed 0 (TFun (TRecord [(''n'', (TPrim (Num U64), Present)), (''stop'', (TFun abbreviatedType4 (TPrim Bool), Present)), (''step'', (TFun abbreviatedType4 abbreviatedType3, Present)), (''acc'', (abbreviatedType3, Present)), (''obsv'', (abbreviatedType2, Present))] Unboxed) abbreviatedType3)"
   apply (unfold abbreviated_type_defs)?
   apply (tactic \<open> map (fn t => DETERM (interpret_tac t @{context} 1)) typing_helper_36_script |> EVERY \<close>)
   done
@@ -642,19 +648,19 @@ val typing_helper_37_script : tac list = [
 
 
 lemma typing_helper_37[unfolded abbreviated_type_defs] :
-  "kinding [] (TFun abbreviatedType6 (TPrim Bool)) {E, S, D}"
+  "kinding [] abbreviatedType1 {E, S, D}"
   apply (unfold abbreviated_type_defs)?
   apply (tactic \<open> map (fn t => DETERM (interpret_tac t @{context} 1)) typing_helper_37_script |> EVERY \<close>)
   done
 
 ML_quiet \<open>
 val typing_helper_38_script : tac list = [
-(ForceTac [])
+(ForceTac [@{thm kinding_def},@{thm kinding_all_def},@{thm kinding_variant_def},@{thm kinding_record_def}])
 ] \<close>
 
 
 lemma typing_helper_38[unfolded abbreviated_type_defs] :
-  "type_wellformed 0 abbreviatedType6"
+  "kinding [] (TRecord [(''p1'', (TPrim (Num U32), Taken)), (''p2'', (TPrim (Num U32), Present))] Unboxed) {E, S, D}"
   apply (unfold abbreviated_type_defs)?
   apply (tactic \<open> map (fn t => DETERM (interpret_tac t @{context} 1)) typing_helper_38_script |> EVERY \<close>)
   done
@@ -666,7 +672,7 @@ val typing_helper_39_script : tac list = [
 
 
 lemma typing_helper_39[unfolded abbreviated_type_defs] :
-  "kinding [] (TFun abbreviatedType6 (TPrim (Num U32))) {E, S, D}"
+  "kinding [] (TRecord [(''p1'', (TPrim (Num U32), Taken)), (''p2'', (TPrim (Num U32), Taken))] Unboxed) {E, S, D}"
   apply (unfold abbreviated_type_defs)?
   apply (tactic \<open> map (fn t => DETERM (interpret_tac t @{context} 1)) typing_helper_39_script |> EVERY \<close>)
   done
@@ -678,7 +684,7 @@ val typing_helper_40_script : tac list = [
 
 
 lemma typing_helper_40[unfolded abbreviated_type_defs] :
-  "kinding [] (TRecord [(''n'', (TPrim (Num U64), Present)), (''stop'', (TFun abbreviatedType6 (TPrim Bool), Present)), (''step'', (TFun abbreviatedType6 (TPrim (Num U32)), Present)), (''acc'', (TPrim (Num U32), Present)), (''obsv'', (TPrim (Num U32), Present))] Unboxed) {E, S, D}"
+  "kinding [] (TFun abbreviatedType7 (TPrim Bool)) {E, S, D}"
   apply (unfold abbreviated_type_defs)?
   apply (tactic \<open> map (fn t => DETERM (interpret_tac t @{context} 1)) typing_helper_40_script |> EVERY \<close>)
   done
@@ -690,19 +696,19 @@ val typing_helper_41_script : tac list = [
 
 
 lemma typing_helper_41[unfolded abbreviated_type_defs] :
-  "type_wellformed 0 (TRecord [(''n'', (TPrim (Num U64), Present)), (''stop'', (TFun abbreviatedType6 (TPrim Bool), Present)), (''step'', (TFun abbreviatedType6 (TPrim (Num U32)), Present)), (''acc'', (TPrim (Num U32), Present)), (''obsv'', (TPrim (Num U32), Present))] Unboxed)"
+  "type_wellformed 0 abbreviatedType7"
   apply (unfold abbreviated_type_defs)?
   apply (tactic \<open> map (fn t => DETERM (interpret_tac t @{context} 1)) typing_helper_41_script |> EVERY \<close>)
   done
 
 ML_quiet \<open>
 val typing_helper_42_script : tac list = [
-(ForceTac [])
+(ForceTac [@{thm kinding_def},@{thm kinding_all_def},@{thm kinding_variant_def},@{thm kinding_record_def}])
 ] \<close>
 
 
 lemma typing_helper_42[unfolded abbreviated_type_defs] :
-  "type_wellformed 0 (TFun (TRecord [(''n'', (TPrim (Num U64), Present)), (''stop'', (TFun abbreviatedType6 (TPrim Bool), Present)), (''step'', (TFun abbreviatedType6 (TPrim (Num U32)), Present)), (''acc'', (TPrim (Num U32), Present)), (''obsv'', (TPrim (Num U32), Present))] Unboxed) (TPrim (Num U32)))"
+  "kinding [] (TFun abbreviatedType7 (TPrim (Num U32))) {E, S, D}"
   apply (unfold abbreviated_type_defs)?
   apply (tactic \<open> map (fn t => DETERM (interpret_tac t @{context} 1)) typing_helper_42_script |> EVERY \<close>)
   done
@@ -714,7 +720,7 @@ val typing_helper_43_script : tac list = [
 
 
 lemma typing_helper_43[unfolded abbreviated_type_defs] :
-  "kinding [] (TFun abbreviatedType5 (TPrim Bool)) {E, S, D}"
+  "kinding [] (TRecord [(''n'', (TPrim (Num U64), Present)), (''stop'', (TFun abbreviatedType7 (TPrim Bool), Present)), (''step'', (TFun abbreviatedType7 (TPrim (Num U32)), Present)), (''acc'', (TPrim (Num U32), Present)), (''obsv'', (TPrim (Num U32), Present))] Unboxed) {E, S, D}"
   apply (unfold abbreviated_type_defs)?
   apply (tactic \<open> map (fn t => DETERM (interpret_tac t @{context} 1)) typing_helper_43_script |> EVERY \<close>)
   done
@@ -726,19 +732,19 @@ val typing_helper_44_script : tac list = [
 
 
 lemma typing_helper_44[unfolded abbreviated_type_defs] :
-  "type_wellformed 0 abbreviatedType5"
+  "type_wellformed 0 (TRecord [(''n'', (TPrim (Num U64), Present)), (''stop'', (TFun abbreviatedType7 (TPrim Bool), Present)), (''step'', (TFun abbreviatedType7 (TPrim (Num U32)), Present)), (''acc'', (TPrim (Num U32), Present)), (''obsv'', (TPrim (Num U32), Present))] Unboxed)"
   apply (unfold abbreviated_type_defs)?
   apply (tactic \<open> map (fn t => DETERM (interpret_tac t @{context} 1)) typing_helper_44_script |> EVERY \<close>)
   done
 
 ML_quiet \<open>
 val typing_helper_45_script : tac list = [
-(ForceTac [@{thm kinding_def},@{thm kinding_all_def},@{thm kinding_variant_def},@{thm kinding_record_def}])
+(ForceTac [])
 ] \<close>
 
 
 lemma typing_helper_45[unfolded abbreviated_type_defs] :
-  "kinding [] (TFun abbreviatedType5 abbreviatedType4) {E, S, D}"
+  "type_wellformed 0 (TFun (TRecord [(''n'', (TPrim (Num U64), Present)), (''stop'', (TFun abbreviatedType7 (TPrim Bool), Present)), (''step'', (TFun abbreviatedType7 (TPrim (Num U32)), Present)), (''acc'', (TPrim (Num U32), Present)), (''obsv'', (TPrim (Num U32), Present))] Unboxed) (TPrim (Num U32)))"
   apply (unfold abbreviated_type_defs)?
   apply (tactic \<open> map (fn t => DETERM (interpret_tac t @{context} 1)) typing_helper_45_script |> EVERY \<close>)
   done
@@ -750,7 +756,7 @@ val typing_helper_46_script : tac list = [
 
 
 lemma typing_helper_46[unfolded abbreviated_type_defs] :
-  "kinding [] (TRecord [(''n'', (TPrim (Num U64), Present)), (''stop'', (TFun abbreviatedType5 (TPrim Bool), Present)), (''step'', (TFun abbreviatedType5 abbreviatedType4, Present)), (''acc'', (abbreviatedType4, Present)), (''obsv'', (TPrim (Num U64), Present))] Unboxed) {E, S, D}"
+  "kinding [] (TFun abbreviatedType6 (TPrim Bool)) {E, S, D}"
   apply (unfold abbreviated_type_defs)?
   apply (tactic \<open> map (fn t => DETERM (interpret_tac t @{context} 1)) typing_helper_46_script |> EVERY \<close>)
   done
@@ -762,21 +768,57 @@ val typing_helper_47_script : tac list = [
 
 
 lemma typing_helper_47[unfolded abbreviated_type_defs] :
-  "type_wellformed 0 (TRecord [(''n'', (TPrim (Num U64), Present)), (''stop'', (TFun abbreviatedType5 (TPrim Bool), Present)), (''step'', (TFun abbreviatedType5 abbreviatedType4, Present)), (''acc'', (abbreviatedType4, Present)), (''obsv'', (TPrim (Num U64), Present))] Unboxed)"
+  "type_wellformed 0 abbreviatedType6"
   apply (unfold abbreviated_type_defs)?
   apply (tactic \<open> map (fn t => DETERM (interpret_tac t @{context} 1)) typing_helper_47_script |> EVERY \<close>)
   done
 
 ML_quiet \<open>
 val typing_helper_48_script : tac list = [
-(ForceTac [])
+(ForceTac [@{thm kinding_def},@{thm kinding_all_def},@{thm kinding_variant_def},@{thm kinding_record_def}])
 ] \<close>
 
 
 lemma typing_helper_48[unfolded abbreviated_type_defs] :
-  "type_wellformed 0 (TFun (TRecord [(''n'', (TPrim (Num U64), Present)), (''stop'', (TFun abbreviatedType5 (TPrim Bool), Present)), (''step'', (TFun abbreviatedType5 abbreviatedType4, Present)), (''acc'', (abbreviatedType4, Present)), (''obsv'', (TPrim (Num U64), Present))] Unboxed) abbreviatedType4)"
+  "kinding [] (TFun abbreviatedType6 abbreviatedType5) {E, S, D}"
   apply (unfold abbreviated_type_defs)?
   apply (tactic \<open> map (fn t => DETERM (interpret_tac t @{context} 1)) typing_helper_48_script |> EVERY \<close>)
+  done
+
+ML_quiet \<open>
+val typing_helper_49_script : tac list = [
+(ForceTac [@{thm kinding_def},@{thm kinding_all_def},@{thm kinding_variant_def},@{thm kinding_record_def}])
+] \<close>
+
+
+lemma typing_helper_49[unfolded abbreviated_type_defs] :
+  "kinding [] (TRecord [(''n'', (TPrim (Num U64), Present)), (''stop'', (TFun abbreviatedType6 (TPrim Bool), Present)), (''step'', (TFun abbreviatedType6 abbreviatedType5, Present)), (''acc'', (abbreviatedType5, Present)), (''obsv'', (TPrim (Num U64), Present))] Unboxed) {E, S, D}"
+  apply (unfold abbreviated_type_defs)?
+  apply (tactic \<open> map (fn t => DETERM (interpret_tac t @{context} 1)) typing_helper_49_script |> EVERY \<close>)
+  done
+
+ML_quiet \<open>
+val typing_helper_50_script : tac list = [
+(ForceTac [])
+] \<close>
+
+
+lemma typing_helper_50[unfolded abbreviated_type_defs] :
+  "type_wellformed 0 (TRecord [(''n'', (TPrim (Num U64), Present)), (''stop'', (TFun abbreviatedType6 (TPrim Bool), Present)), (''step'', (TFun abbreviatedType6 abbreviatedType5, Present)), (''acc'', (abbreviatedType5, Present)), (''obsv'', (TPrim (Num U64), Present))] Unboxed)"
+  apply (unfold abbreviated_type_defs)?
+  apply (tactic \<open> map (fn t => DETERM (interpret_tac t @{context} 1)) typing_helper_50_script |> EVERY \<close>)
+  done
+
+ML_quiet \<open>
+val typing_helper_51_script : tac list = [
+(ForceTac [])
+] \<close>
+
+
+lemma typing_helper_51[unfolded abbreviated_type_defs] :
+  "type_wellformed 0 (TFun (TRecord [(''n'', (TPrim (Num U64), Present)), (''stop'', (TFun abbreviatedType6 (TPrim Bool), Present)), (''step'', (TFun abbreviatedType6 abbreviatedType5, Present)), (''acc'', (abbreviatedType5, Present)), (''obsv'', (TPrim (Num U64), Present))] Unboxed) abbreviatedType5)"
+  apply (unfold abbreviated_type_defs)?
+  apply (tactic \<open> map (fn t => DETERM (interpret_tac t @{context} 1)) typing_helper_51_script |> EVERY \<close>)
   done
 
 ML_quiet \<open>
@@ -897,35 +939,13 @@ StepUp,
 Val (TypingTacs []),
 Val (KindingTacs [(RTac @{thm typing_helper_17})]),
 StepDown,
-StepDown,
-Val (KindingTacs [(RTac @{thm typing_helper_14})]),
-Val (KindingTacs [(RTac @{thm typing_helper_19})]),
-StepUp,
 Val (TypingTacs []),
-Val (KindingTacs [(RTac @{thm typing_helper_14})]),
 StepDown,
-StepDown,
-Val (KindingTacs [(RTac @{thm typing_helper_14})]),
-StepUp,
-Val (TypingTacs [(RTac @{thm typing_app}),(SplitsTac [SOME [(RTac @{thm split_comp.left}),(RTac @{thm type_wellformed_prettyI}),(SimpTac ([],@{thms type_wellformed.simps})),(RTac @{thm typing_helper_20})],SOME [(RTac @{thm split_comp.left}),(RTac @{thm type_wellformed_prettyI}),(SimpTac ([],@{thms type_wellformed.simps})),(RTac @{thm typing_helper_21})],SOME [(RTac @{thm split_comp.right}),(RTac @{thm type_wellformed_prettyI}),(SimpTac ([],@{thms type_wellformed.simps})),(RTac @{thm typing_helper_22})],NONE]),(RTac @{thm typing_afun'}),(SimpTac ([@{thm \<Xi>_def},@{thm wordarray_length_0_type_def[unfolded abbreviated_type_defs]}],[])),(RTac @{thm typing_helper_23}),(SimpSolveTac ([],[])),(SimpSolveTac ([],[])),(RTac @{thm type_wellformed_prettyI}),(SimpTac ([],@{thms type_wellformed.simps})),(RTac @{thm typing_helper_24}),(SimpTac ([@{thm empty_def}],[])),(WeakeningTac [@{thm typing_helper_14},@{thm typing_helper_19}]),(RTac @{thm typing_var}),(SimpTac ([@{thm empty_def}],[])),(WeakeningTac [@{thm typing_helper_17}]),(SimpSolveTac ([],[]))]),
-StepDown,
-StepDown,
-Val (KindingTacs [(RTac @{thm typing_helper_14})]),
 StepUp,
 Val (TypingTacs [(RTac @{thm typing_lit'}),(SimpTac ([@{thm empty_def}],[])),(WeakeningTac [@{thm typing_helper_14}]),(SimpSolveTac ([],[]))]),
 StepDown,
 StepDown,
-Val (KindingTacs [(RTac @{thm typing_helper_25})]),
-StepUp,
-Val (TypingTacs []),
-StepDown,
-StepDown,
-Val (KindingTacs [(RTac @{thm typing_helper_14})]),
-StepUp,
-Val (TypingTacs [(RTac @{thm typing_app}),(SplitsTac [SOME [(RTac @{thm split_comp.right}),(RTac @{thm type_wellformed_prettyI}),(SimpTac ([],@{thms type_wellformed.simps})),(RTac @{thm typing_helper_26})],NONE]),(RTac @{thm typing_afun'}),(SimpTac ([@{thm \<Xi>_def},@{thm wordarray_get_0_type_def[unfolded abbreviated_type_defs]}],[])),(RTac @{thm typing_helper_23}),(SimpSolveTac ([],[])),(SimpSolveTac ([],[])),(RTac @{thm type_wellformed_prettyI}),(SimpTac ([],@{thms type_wellformed.simps})),(RTac @{thm typing_helper_27}),(SimpTac ([@{thm empty_def}],[])),(WeakeningTac []),(RTac @{thm typing_var}),(SimpTac ([@{thm empty_def}],[])),(WeakeningTac [@{thm typing_helper_25}]),(SimpSolveTac ([],[]))]),
-StepDown,
-StepDown,
-Val (KindingTacs [(RTac @{thm typing_helper_28})]),
+Val (KindingTacs [(RTac @{thm typing_helper_17})]),
 StepUp,
 Val (TypingTacs []),
 StepDown,
@@ -934,10 +954,6 @@ StepDown,
 StepUp,
 Val (TypingTacs [(RTac @{thm typing_lit'}),(SimpTac ([@{thm empty_def}],[])),(WeakeningTac []),(SimpSolveTac ([],[]))]),
 Val (TypingTacs [(RTac @{thm typing_lit'}),(SimpTac ([@{thm empty_def}],[])),(WeakeningTac []),(SimpSolveTac ([],[]))]),
-StepUp,
-StepUp,
-StepUp,
-StepUp,
 StepUp,
 StepUp,
 StepUp,
@@ -968,14 +984,14 @@ Val (KindingTacs [(RTac @{thm typing_helper_1})]),
 StepDown,
 StepDown,
 Val (KindingTacs [(RTac @{thm typing_helper_14})]),
-Val (KindingTacs [(RTac @{thm typing_helper_29})]),
+Val (KindingTacs [(RTac @{thm typing_helper_19})]),
 StepUp,
 Val (TypingTacs []),
 Val (KindingTacs [(RTac @{thm typing_helper_14})]),
 StepDown,
 StepDown,
 Val (KindingTacs [(RTac @{thm typing_helper_14})]),
-Val (KindingTacs [(RTac @{thm typing_helper_30})]),
+Val (KindingTacs [(RTac @{thm typing_helper_20})]),
 StepUp,
 Val (TypingTacs []),
 Val (KindingTacs [(RTac @{thm typing_helper_14})]),
@@ -1114,8 +1130,15 @@ Val (TypingTacs []),
 Val (KindingTacs [(RTac @{thm typing_helper_17})]),
 StepDown,
 StepDown,
+Val (KindingTacs [(RTac @{thm typing_helper_21})]),
+Val (KindingTacs [(RTac @{thm typing_helper_22})]),
+StepUp,
+Val (TypingTacs []),
+Val (KindingTacs [(RTac @{thm typing_helper_21})]),
+StepDown,
+StepDown,
 Val (KindingTacs [(RTac @{thm typing_helper_14})]),
-Val (KindingTacs [(RTac @{thm typing_helper_19})]),
+Val (KindingTacs [(RTac @{thm typing_helper_23})]),
 StepUp,
 Val (TypingTacs []),
 Val (KindingTacs [(RTac @{thm typing_helper_14})]),
@@ -1146,17 +1169,17 @@ StepUp,
 Val (TypingTacs [(RTac @{thm typing_lit'}),(SimpTac ([@{thm empty_def}],[])),(WeakeningTac []),(SimpSolveTac ([],[]))]),
 StepDown,
 StepDown,
-Val (KindingTacs [(RTac @{thm typing_helper_25})]),
+Val (KindingTacs [(RTac @{thm typing_helper_24})]),
 StepUp,
 Val (TypingTacs []),
 StepDown,
 StepDown,
 Val (KindingTacs [(RTac @{thm typing_helper_14})]),
 StepUp,
-Val (TypingTacs [(RTac @{thm typing_app}),(SplitsTac [SOME [(RTac @{thm split_comp.right}),(RTac @{thm type_wellformed_prettyI}),(SimpTac ([],@{thms type_wellformed.simps})),(RTac @{thm typing_helper_26})],NONE]),(RTac @{thm typing_afun'}),(SimpTac ([@{thm \<Xi>_def},@{thm wordarray_get_0_type_def[unfolded abbreviated_type_defs]}],[])),(RTac @{thm typing_helper_23}),(SimpSolveTac ([],[])),(SimpSolveTac ([],[])),(RTac @{thm type_wellformed_prettyI}),(SimpTac ([],@{thms type_wellformed.simps})),(RTac @{thm typing_helper_27}),(SimpTac ([@{thm empty_def}],[])),(WeakeningTac []),(RTac @{thm typing_var}),(SimpTac ([@{thm empty_def}],[])),(WeakeningTac [@{thm typing_helper_25}]),(SimpSolveTac ([],[]))]),
+Val (TypingTacs [(RTac @{thm typing_app}),(SplitsTac [SOME [(RTac @{thm split_comp.right}),(RTac @{thm type_wellformed_prettyI}),(SimpTac ([],@{thms type_wellformed.simps})),(RTac @{thm typing_helper_25})],NONE]),(RTac @{thm typing_afun'}),(SimpTac ([@{thm \<Xi>_def},@{thm wordarray_get_0_type_def[unfolded abbreviated_type_defs]}],[])),(RTac @{thm typing_helper_26}),(SimpSolveTac ([],[])),(SimpSolveTac ([],[])),(RTac @{thm type_wellformed_prettyI}),(SimpTac ([],@{thms type_wellformed.simps})),(RTac @{thm typing_helper_27}),(SimpTac ([@{thm empty_def}],[])),(WeakeningTac []),(RTac @{thm typing_var}),(SimpTac ([@{thm empty_def}],[])),(WeakeningTac [@{thm typing_helper_24}]),(SimpSolveTac ([],[]))]),
 StepDown,
 StepDown,
-Val (KindingTacs [(RTac @{thm typing_helper_28})]),
+Val (KindingTacs [(RTac @{thm typing_helper_17})]),
 StepUp,
 Val (TypingTacs []),
 StepDown,
@@ -1176,7 +1199,26 @@ Val (TypingTacs []),
 Val (TypingTacs []),
 StepUp,
 StepUp,
+StepDown,
+StepDown,
+Val (KindingTacs [(RTac @{thm typing_helper_17})]),
+StepUp,
 Val (TypingTacs []),
+StepDown,
+Val (TypingTacs []),
+StepDown,
+StepUp,
+Val (TypingTacs []),
+StepDown,
+StepDown,
+Val (KindingTacs [(RTac @{thm typing_helper_17})]),
+StepUp,
+Val (TypingTacs [(RTac @{thm typing_lit'}),(SimpTac ([@{thm empty_def}],[])),(WeakeningTac [@{thm typing_helper_17},@{thm typing_helper_14}]),(SimpSolveTac ([],[]))]),
+Val (TypingTacs []),
+StepUp,
+StepUp,
+StepUp,
+StepUp,
 StepUp,
 StepUp,
 StepUp,
@@ -1213,15 +1255,15 @@ StepDown,
 Val (KindingTacs [(RTac @{thm typing_helper_12})]),
 StepDown,
 StepDown,
-Val (KindingTacs [(RTac @{thm typing_helper_17})]),
-Val (KindingTacs [(RTac @{thm typing_helper_18})]),
+Val (KindingTacs [(RTac @{thm typing_helper_21})]),
+Val (KindingTacs [(RTac @{thm typing_helper_22})]),
 StepUp,
 Val (TypingTacs []),
-Val (KindingTacs [(RTac @{thm typing_helper_17})]),
+Val (KindingTacs [(RTac @{thm typing_helper_21})]),
 StepDown,
 StepDown,
 Val (KindingTacs [(RTac @{thm typing_helper_14})]),
-Val (KindingTacs [(RTac @{thm typing_helper_19})]),
+Val (KindingTacs [(RTac @{thm typing_helper_23})]),
 StepUp,
 Val (TypingTacs []),
 Val (KindingTacs [(RTac @{thm typing_helper_14})]),
@@ -1229,7 +1271,7 @@ StepDown,
 StepDown,
 Val (KindingTacs [(RTac @{thm typing_helper_14})]),
 StepUp,
-Val (TypingTacs [(RTac @{thm typing_app}),(SplitsTac [NONE,SOME [(RTac @{thm split_comp.left}),(RTac @{thm type_wellformed_prettyI}),(SimpTac ([],@{thms type_wellformed.simps})),(RTac @{thm typing_helper_21})],SOME [(RTac @{thm split_comp.right}),(RTac @{thm type_wellformed_prettyI}),(SimpTac ([],@{thms type_wellformed.simps})),(RTac @{thm typing_helper_22})],NONE]),(RTac @{thm typing_afun'}),(SimpTac ([@{thm \<Xi>_def},@{thm wordarray_length_0_type_def[unfolded abbreviated_type_defs]}],[])),(RTac @{thm typing_helper_23}),(SimpSolveTac ([],[])),(SimpSolveTac ([],[])),(RTac @{thm type_wellformed_prettyI}),(SimpTac ([],@{thms type_wellformed.simps})),(RTac @{thm typing_helper_24}),(SimpTac ([@{thm empty_def}],[])),(WeakeningTac [@{thm typing_helper_19}]),(RTac @{thm typing_var}),(SimpTac ([@{thm empty_def}],[])),(WeakeningTac [@{thm typing_helper_17}]),(SimpSolveTac ([],[]))]),
+Val (TypingTacs [(RTac @{thm typing_app}),(SplitsTac [NONE,SOME [(RTac @{thm split_comp.left}),(RTac @{thm type_wellformed_prettyI}),(SimpTac ([],@{thms type_wellformed.simps})),(RTac @{thm typing_helper_28})],SOME [(RTac @{thm split_comp.right}),(RTac @{thm type_wellformed_prettyI}),(SimpTac ([],@{thms type_wellformed.simps})),(RTac @{thm typing_helper_29})],NONE]),(RTac @{thm typing_afun'}),(SimpTac ([@{thm \<Xi>_def},@{thm wordarray_length_0_type_def[unfolded abbreviated_type_defs]}],[])),(RTac @{thm typing_helper_26}),(SimpSolveTac ([],[])),(SimpSolveTac ([],[])),(RTac @{thm type_wellformed_prettyI}),(SimpTac ([],@{thms type_wellformed.simps})),(RTac @{thm typing_helper_30}),(SimpTac ([@{thm empty_def}],[])),(WeakeningTac [@{thm typing_helper_23}]),(RTac @{thm typing_var}),(SimpTac ([@{thm empty_def}],[])),(WeakeningTac [@{thm typing_helper_21}]),(SimpSolveTac ([],[]))]),
 StepDown,
 StepDown,
 Val (KindingTacs [(RTac @{thm typing_helper_5})]),
@@ -1239,15 +1281,20 @@ StepDown,
 StepDown,
 Val (KindingTacs [(RTac @{thm typing_helper_31})]),
 StepUp,
-Val (TypingTacs [(RTac @{thm typing_fun'}),(RTac @{thm searchStop_typecorrect[simplified searchStop_type_def searchStop_typetree_def abbreviated_type_defs, simplified]}),(RTac @{thm typing_helper_23}),(SimpSolveTac ([],[])),(SimpSolveTac ([],[])),(RTac @{thm type_wellformed_prettyI}),(SimpTac ([],@{thms type_wellformed.simps})),(RTac @{thm typing_helper_32}),(SimpTac ([@{thm empty_def}],[])),(WeakeningTac [])]),
+Val (TypingTacs [(RTac @{thm typing_fun'}),(RTac @{thm searchStop_typecorrect[simplified searchStop_type_def searchStop_typetree_def abbreviated_type_defs, simplified]}),(RTac @{thm typing_helper_26}),(SimpSolveTac ([],[])),(SimpSolveTac ([],[])),(RTac @{thm type_wellformed_prettyI}),(SimpTac ([],@{thms type_wellformed.simps})),(RTac @{thm typing_helper_32}),(SimpTac ([@{thm empty_def}],[])),(WeakeningTac [])]),
 StepDown,
 StepDown,
 Val (KindingTacs [(RTac @{thm typing_helper_33})]),
 StepUp,
-Val (TypingTacs [(RTac @{thm typing_fun'}),(RTac @{thm searchNext_typecorrect[simplified searchNext_type_def searchNext_typetree_def abbreviated_type_defs, simplified]}),(RTac @{thm typing_helper_23}),(SimpSolveTac ([],[])),(SimpSolveTac ([],[])),(RTac @{thm type_wellformed_prettyI}),(SimpTac ([],@{thms type_wellformed.simps})),(RTac @{thm typing_helper_32}),(SimpTac ([@{thm empty_def}],[])),(WeakeningTac [])]),
+Val (TypingTacs [(RTac @{thm typing_fun'}),(RTac @{thm searchNext_typecorrect[simplified searchNext_type_def searchNext_typetree_def abbreviated_type_defs, simplified]}),(RTac @{thm typing_helper_26}),(SimpSolveTac ([],[])),(SimpSolveTac ([],[])),(RTac @{thm type_wellformed_prettyI}),(SimpTac ([],@{thms type_wellformed.simps})),(RTac @{thm typing_helper_32}),(SimpTac ([@{thm empty_def}],[])),(WeakeningTac [])]),
 StepDown,
 StepDown,
 Val (KindingTacs [(RTac @{thm typing_helper_14})]),
+StepUp,
+Val (TypingTacs [(RTac @{thm typing_lit'}),(SimpTac ([@{thm empty_def}],[])),(WeakeningTac []),(SimpSolveTac ([],[]))]),
+StepDown,
+StepDown,
+Val (KindingTacs [(RTac @{thm typing_helper_17})]),
 StepUp,
 Val (TypingTacs [(RTac @{thm typing_lit'}),(SimpTac ([@{thm empty_def}],[])),(WeakeningTac []),(SimpSolveTac ([],[]))]),
 StepDown,
@@ -1269,7 +1316,7 @@ StepDown,
 StepDown,
 Val (KindingTacs [(RTac @{thm typing_helper_10})]),
 StepUp,
-Val (TypingTacs [(RTac @{thm typing_app}),(SplitsTac [SOME [(RTac @{thm split_comp.right}),(RTac @{thm type_wellformed_prettyI}),(SimpTac ([],@{thms type_wellformed.simps})),(RTac @{thm typing_helper_35})],NONE]),(RTac @{thm typing_afun'}),(SimpTac ([@{thm \<Xi>_def},@{thm repeat_2_type_def[unfolded abbreviated_type_defs]}],[])),(RTac @{thm typing_helper_23}),(SimpSolveTac ([],[])),(SimpSolveTac ([],[])),(RTac @{thm type_wellformed_prettyI}),(SimpTac ([],@{thms type_wellformed.simps})),(RTac @{thm typing_helper_36}),(SimpTac ([@{thm empty_def}],[])),(WeakeningTac []),(RTac @{thm typing_var}),(SimpTac ([@{thm empty_def}],[])),(WeakeningTac [@{thm typing_helper_34}]),(SimpSolveTac ([],[]))]),
+Val (TypingTacs [(RTac @{thm typing_app}),(SplitsTac [SOME [(RTac @{thm split_comp.right}),(RTac @{thm type_wellformed_prettyI}),(SimpTac ([],@{thms type_wellformed.simps})),(RTac @{thm typing_helper_35})],NONE]),(RTac @{thm typing_afun'}),(SimpTac ([@{thm \<Xi>_def},@{thm repeat_2_type_def[unfolded abbreviated_type_defs]}],[])),(RTac @{thm typing_helper_26}),(SimpSolveTac ([],[])),(SimpSolveTac ([],[])),(RTac @{thm type_wellformed_prettyI}),(SimpTac ([],@{thms type_wellformed.simps})),(RTac @{thm typing_helper_36}),(SimpTac ([@{thm empty_def}],[])),(WeakeningTac []),(RTac @{thm typing_var}),(SimpTac ([@{thm empty_def}],[])),(WeakeningTac [@{thm typing_helper_34}]),(SimpSolveTac ([],[]))]),
 StepDown,
 StepDown,
 Val (KindingTacs [(RTac @{thm typing_helper_14})]),
@@ -1284,7 +1331,22 @@ Val (KindingTacs [(RTac @{thm typing_helper_16})]),
 StepUp,
 Val (TypingTacs []),
 Val (KindingTacs [(RTac @{thm typing_helper_14})]),
+StepDown,
+StepDown,
+Val (KindingTacs [(RTac @{thm typing_helper_17})]),
+Val (KindingTacs [(RTac @{thm typing_helper_18})]),
+StepUp,
 Val (TypingTacs []),
+Val (KindingTacs [(RTac @{thm typing_helper_17})]),
+StepDown,
+Val (TypingTacs []),
+StepDown,
+StepUp,
+Val (TypingTacs []),
+Val (TypingTacs []),
+StepUp,
+StepUp,
+StepUp,
 StepUp,
 StepUp,
 StepUp,
@@ -1316,18 +1378,18 @@ lemma binarySearch_typecorrect :
 ML_quiet \<open>
 val myexp_typecorrect_script : hints treestep list = [
 StepDown,
-Val (KindingTacs [(RTac @{thm typing_helper_10})]),
+Val (KindingTacs [(RTac @{thm typing_helper_37})]),
 StepDown,
 StepDown,
 Val (KindingTacs [(RTac @{thm typing_helper_14})]),
-Val (KindingTacs [(RTac @{thm typing_helper_15})]),
+Val (KindingTacs [(RTac @{thm typing_helper_38})]),
 StepUp,
 Val (TypingTacs []),
 Val (KindingTacs [(RTac @{thm typing_helper_14})]),
 StepDown,
 StepDown,
 Val (KindingTacs [(RTac @{thm typing_helper_14})]),
-Val (KindingTacs [(RTac @{thm typing_helper_16})]),
+Val (KindingTacs [(RTac @{thm typing_helper_39})]),
 StepUp,
 Val (TypingTacs []),
 Val (KindingTacs [(RTac @{thm typing_helper_14})]),
@@ -1335,17 +1397,17 @@ StepDown,
 StepDown,
 Val (KindingTacs [(RTac @{thm typing_helper_5})]),
 StepUp,
-Val (TypingTacs [(RTac @{thm typing_cast}),(RTac @{thm typing_var}),(SimpTac ([@{thm empty_def}],[])),(WeakeningTac [@{thm typing_helper_14},@{thm typing_helper_16}]),(SimpSolveTac ([],[])),(SimpSolveTac ([],[]))]),
+Val (TypingTacs [(RTac @{thm typing_cast}),(RTac @{thm typing_var}),(SimpTac ([@{thm empty_def}],[])),(WeakeningTac [@{thm typing_helper_14},@{thm typing_helper_39}]),(SimpSolveTac ([],[])),(SimpSolveTac ([],[]))]),
 StepDown,
 StepDown,
-Val (KindingTacs [(RTac @{thm typing_helper_37})]),
+Val (KindingTacs [(RTac @{thm typing_helper_40})]),
 StepUp,
-Val (TypingTacs [(RTac @{thm typing_fun'}),(RTac @{thm expstop_typecorrect[simplified expstop_type_def expstop_typetree_def abbreviated_type_defs, simplified]}),(RTac @{thm typing_helper_23}),(SimpSolveTac ([],[])),(SimpSolveTac ([],[])),(RTac @{thm type_wellformed_prettyI}),(SimpTac ([],@{thms type_wellformed.simps})),(RTac @{thm typing_helper_38}),(SimpTac ([@{thm empty_def}],[])),(WeakeningTac [])]),
+Val (TypingTacs [(RTac @{thm typing_fun'}),(RTac @{thm expstop_typecorrect[simplified expstop_type_def expstop_typetree_def abbreviated_type_defs, simplified]}),(RTac @{thm typing_helper_26}),(SimpSolveTac ([],[])),(SimpSolveTac ([],[])),(RTac @{thm type_wellformed_prettyI}),(SimpTac ([],@{thms type_wellformed.simps})),(RTac @{thm typing_helper_41}),(SimpTac ([@{thm empty_def}],[])),(WeakeningTac [])]),
 StepDown,
 StepDown,
-Val (KindingTacs [(RTac @{thm typing_helper_39})]),
+Val (KindingTacs [(RTac @{thm typing_helper_42})]),
 StepUp,
-Val (TypingTacs [(RTac @{thm typing_fun'}),(RTac @{thm expstep_typecorrect[simplified expstep_type_def expstep_typetree_def abbreviated_type_defs, simplified]}),(RTac @{thm typing_helper_23}),(SimpSolveTac ([],[])),(SimpSolveTac ([],[])),(RTac @{thm type_wellformed_prettyI}),(SimpTac ([],@{thms type_wellformed.simps})),(RTac @{thm typing_helper_38}),(SimpTac ([@{thm empty_def}],[])),(WeakeningTac [])]),
+Val (TypingTacs [(RTac @{thm typing_fun'}),(RTac @{thm expstep_typecorrect[simplified expstep_type_def expstep_typetree_def abbreviated_type_defs, simplified]}),(RTac @{thm typing_helper_26}),(SimpSolveTac ([],[])),(SimpSolveTac ([],[])),(RTac @{thm type_wellformed_prettyI}),(SimpTac ([],@{thms type_wellformed.simps})),(RTac @{thm typing_helper_41}),(SimpTac ([@{thm empty_def}],[])),(WeakeningTac [])]),
 StepDown,
 StepDown,
 Val (KindingTacs [(RTac @{thm typing_helper_14})]),
@@ -1353,10 +1415,10 @@ StepUp,
 Val (TypingTacs [(RTac @{thm typing_lit'}),(SimpTac ([@{thm empty_def}],[])),(WeakeningTac []),(SimpSolveTac ([],[]))]),
 StepDown,
 StepDown,
-Val (KindingTacs [(RTac @{thm typing_helper_40})]),
+Val (KindingTacs [(RTac @{thm typing_helper_43})]),
 StepUp,
 Val (TypingTacs []),
-Val (TypingTacs [(RTac @{thm typing_app}),(SplitsTac [SOME [(RTac @{thm split_comp.right}),(RTac @{thm type_wellformed_prettyI}),(SimpTac ([],@{thms type_wellformed.simps})),(RTac @{thm typing_helper_41})],NONE]),(RTac @{thm typing_afun'}),(SimpTac ([@{thm \<Xi>_def},@{thm repeat_1_type_def[unfolded abbreviated_type_defs]}],[])),(RTac @{thm typing_helper_23}),(SimpSolveTac ([],[])),(SimpSolveTac ([],[])),(RTac @{thm type_wellformed_prettyI}),(SimpTac ([],@{thms type_wellformed.simps})),(RTac @{thm typing_helper_42}),(SimpTac ([@{thm empty_def}],[])),(WeakeningTac []),(RTac @{thm typing_var}),(SimpTac ([@{thm empty_def}],[])),(WeakeningTac [@{thm typing_helper_40}]),(SimpSolveTac ([],[]))]),
+Val (TypingTacs [(RTac @{thm typing_app}),(SplitsTac [SOME [(RTac @{thm split_comp.right}),(RTac @{thm type_wellformed_prettyI}),(SimpTac ([],@{thms type_wellformed.simps})),(RTac @{thm typing_helper_44})],NONE]),(RTac @{thm typing_afun'}),(SimpTac ([@{thm \<Xi>_def},@{thm repeat_1_type_def[unfolded abbreviated_type_defs]}],[])),(RTac @{thm typing_helper_26}),(SimpSolveTac ([],[])),(SimpSolveTac ([],[])),(RTac @{thm type_wellformed_prettyI}),(SimpTac ([],@{thms type_wellformed.simps})),(RTac @{thm typing_helper_45}),(SimpTac ([@{thm empty_def}],[])),(WeakeningTac []),(RTac @{thm typing_var}),(SimpTac ([@{thm empty_def}],[])),(WeakeningTac [@{thm typing_helper_43}]),(SimpSolveTac ([],[]))]),
 StepUp,
 StepUp,
 StepUp,
@@ -1390,39 +1452,39 @@ StepUp,
 Val (TypingTacs []),
 StepDown,
 StepDown,
-Val (KindingTacs [(RTac @{thm typing_helper_43})]),
-StepUp,
-Val (TypingTacs [(RTac @{thm typing_fun'}),(RTac @{thm log2stop_typecorrect[simplified log2stop_type_def log2stop_typetree_def abbreviated_type_defs, simplified]}),(RTac @{thm typing_helper_23}),(SimpSolveTac ([],[])),(SimpSolveTac ([],[])),(RTac @{thm type_wellformed_prettyI}),(SimpTac ([],@{thms type_wellformed.simps})),(RTac @{thm typing_helper_44}),(SimpTac ([@{thm empty_def}],[])),(WeakeningTac [])]),
-StepDown,
-StepDown,
-Val (KindingTacs [(RTac @{thm typing_helper_45})]),
-StepUp,
-Val (TypingTacs [(RTac @{thm typing_fun'}),(RTac @{thm log2step_typecorrect[simplified log2step_type_def log2step_typetree_def abbreviated_type_defs, simplified]}),(RTac @{thm typing_helper_23}),(SimpSolveTac ([],[])),(SimpSolveTac ([],[])),(RTac @{thm type_wellformed_prettyI}),(SimpTac ([],@{thms type_wellformed.simps})),(RTac @{thm typing_helper_44}),(SimpTac ([@{thm empty_def}],[])),(WeakeningTac [])]),
-StepDown,
-StepDown,
-Val (KindingTacs [(RTac @{thm typing_helper_5})]),
-StepUp,
-Val (TypingTacs [(RTac @{thm typing_lit'}),(SimpTac ([@{thm empty_def}],[])),(WeakeningTac []),(SimpSolveTac ([],[]))]),
-StepDown,
-StepDown,
-Val (KindingTacs [(RTac @{thm typing_helper_5})]),
-StepUp,
-Val (TypingTacs [(RTac @{thm typing_lit'}),(SimpTac ([@{thm empty_def}],[])),(WeakeningTac []),(SimpSolveTac ([],[]))]),
-StepDown,
-StepDown,
-Val (KindingTacs [(RTac @{thm typing_helper_3})]),
-StepUp,
-Val (TypingTacs []),
-StepDown,
-StepDown,
 Val (KindingTacs [(RTac @{thm typing_helper_46})]),
 StepUp,
+Val (TypingTacs [(RTac @{thm typing_fun'}),(RTac @{thm log2stop_typecorrect[simplified log2stop_type_def log2stop_typetree_def abbreviated_type_defs, simplified]}),(RTac @{thm typing_helper_26}),(SimpSolveTac ([],[])),(SimpSolveTac ([],[])),(RTac @{thm type_wellformed_prettyI}),(SimpTac ([],@{thms type_wellformed.simps})),(RTac @{thm typing_helper_47}),(SimpTac ([@{thm empty_def}],[])),(WeakeningTac [])]),
+StepDown,
+StepDown,
+Val (KindingTacs [(RTac @{thm typing_helper_48})]),
+StepUp,
+Val (TypingTacs [(RTac @{thm typing_fun'}),(RTac @{thm log2step_typecorrect[simplified log2step_type_def log2step_typetree_def abbreviated_type_defs, simplified]}),(RTac @{thm typing_helper_26}),(SimpSolveTac ([],[])),(SimpSolveTac ([],[])),(RTac @{thm type_wellformed_prettyI}),(SimpTac ([],@{thms type_wellformed.simps})),(RTac @{thm typing_helper_47}),(SimpTac ([@{thm empty_def}],[])),(WeakeningTac [])]),
+StepDown,
+StepDown,
+Val (KindingTacs [(RTac @{thm typing_helper_5})]),
+StepUp,
+Val (TypingTacs [(RTac @{thm typing_lit'}),(SimpTac ([@{thm empty_def}],[])),(WeakeningTac []),(SimpSolveTac ([],[]))]),
+StepDown,
+StepDown,
+Val (KindingTacs [(RTac @{thm typing_helper_5})]),
+StepUp,
+Val (TypingTacs [(RTac @{thm typing_lit'}),(SimpTac ([@{thm empty_def}],[])),(WeakeningTac []),(SimpSolveTac ([],[]))]),
+StepDown,
+StepDown,
+Val (KindingTacs [(RTac @{thm typing_helper_3})]),
+StepUp,
+Val (TypingTacs []),
+StepDown,
+StepDown,
+Val (KindingTacs [(RTac @{thm typing_helper_49})]),
+StepUp,
 Val (TypingTacs []),
 StepDown,
 StepDown,
 Val (KindingTacs [(RTac @{thm typing_helper_3})]),
 StepUp,
-Val (TypingTacs [(RTac @{thm typing_app}),(SplitsTac [SOME [(RTac @{thm split_comp.right}),(RTac @{thm type_wellformed_prettyI}),(SimpTac ([],@{thms type_wellformed.simps})),(RTac @{thm typing_helper_47})],NONE]),(RTac @{thm typing_afun'}),(SimpTac ([@{thm \<Xi>_def},@{thm repeat_0_type_def[unfolded abbreviated_type_defs]}],[])),(RTac @{thm typing_helper_23}),(SimpSolveTac ([],[])),(SimpSolveTac ([],[])),(RTac @{thm type_wellformed_prettyI}),(SimpTac ([],@{thms type_wellformed.simps})),(RTac @{thm typing_helper_48}),(SimpTac ([@{thm empty_def}],[])),(WeakeningTac []),(RTac @{thm typing_var}),(SimpTac ([@{thm empty_def}],[])),(WeakeningTac [@{thm typing_helper_46}]),(SimpSolveTac ([],[]))]),
+Val (TypingTacs [(RTac @{thm typing_app}),(SplitsTac [SOME [(RTac @{thm split_comp.right}),(RTac @{thm type_wellformed_prettyI}),(SimpTac ([],@{thms type_wellformed.simps})),(RTac @{thm typing_helper_50})],NONE]),(RTac @{thm typing_afun'}),(SimpTac ([@{thm \<Xi>_def},@{thm repeat_0_type_def[unfolded abbreviated_type_defs]}],[])),(RTac @{thm typing_helper_26}),(SimpSolveTac ([],[])),(SimpSolveTac ([],[])),(RTac @{thm type_wellformed_prettyI}),(SimpTac ([],@{thms type_wellformed.simps})),(RTac @{thm typing_helper_51}),(SimpTac ([@{thm empty_def}],[])),(WeakeningTac []),(RTac @{thm typing_var}),(SimpTac ([@{thm empty_def}],[])),(WeakeningTac [@{thm typing_helper_49}]),(SimpSolveTac ([],[]))]),
 StepDown,
 StepDown,
 Val (KindingTacs [(RTac @{thm typing_helper_5})]),
